LN/Multisorted/Theory.v
@@ -3,8 +3,7 @@
 From Tealeaves Require Import
      Util.Prelude
      Util.EqDec_eq LN.Atom LN.AtomSet
-     LN.Multisorted.Operations
-     LN.Multisorted.OperationsEq.
+     LN.Multisorted.Operations.
 
 From Multisorted Require Import
      Classes.DTM
@@ -19,6 +18,297 @@ Import DTMContainer.Notations.
 #[local] Open Scope tealeaves_scope.
 #[local] Open Scope tealeaves_multi_scope.
 #[local] Open Scope set_scope.
+#[local] Open Scope nat_scope. (* Let <<x + y>> be addition, not sum type. *)
+
+(** * Basic specifications for <<open>>, <<close>>, and <<subst>> *)
+(******************************************************************************)
+Section operations_specifications.
+
+  Context
+    (S : Type -> Type)
+    `{DTPreModule (list K) S T (mn_op := Monoid_op_list) (mn_unit := Monoid_unit_list)}
+    `{! DTM (list K) T}.
+
+  Implicit Types (l : leaf) (w : list K) (t : S leaf) (x : atom).
+
+  (** ** Identity and equality lemmas for operations *)
+  (******************************************************************************)
+
+  (** *** For [open] *)
+  (******************************************************************************)
+  Lemma open_eq : forall k t (u1 u2 : T k leaf),
+      (forall (w : list K) (l : leaf), (w, (k, l)) ∈md t -> open_loc k u1 (w, l) = open_loc k u2 (w, l)) ->
+      t '(k | u1) = t '(k | u2).
+  Proof.
+    introv hyp. unfold open. apply kbindd_respectful. auto.
+  Qed.
+
+  Lemma open_id : forall k t u,
+      (forall w l, (w, (k, l)) ∈md t -> open_loc k u (w, l) = mret T k l) ->
+      t '(k | u) = t.
+  Proof.
+    intros. unfold open.
+    now apply (kbindd_respectful_id k).
+  Qed.
+
+  (** *** For [subst] *)
+  (******************************************************************************)
+  Lemma subst_eq : forall k t x u1 u2,
+      (forall l, (k, l) ∈m t -> subst_loc k x u1 l = subst_loc k x u2 l) ->
+      t '{k | x ~> u1} = t '{k | x ~> u2}.
+  Proof.
+    introv hyp. unfold subst. apply kbind_respectful. auto.
+  Qed.
+
+  Lemma subst_id : forall k t x u,
+      (forall l, (k, l) ∈m t -> subst_loc k x u l = mret T k l) ->
+      t '{k | x ~> u} = t.
+  Proof.
+    intros. unfold subst.
+    now apply kbind_respectful_id.
+  Qed.
+
+  (** *** For [close] *)
+  (******************************************************************************)
+  Lemma close_eq : forall k t x y,
+      (forall w l, (w, (k, l)) ∈md t -> close_loc k x (w, l) = close_loc k y (w, l)) ->
+      '[k | x] t = '[k | y] t.
+  Proof.
+    intros. unfold close.
+    now apply (kfmapd_respectful).
+  Qed.
+
+  Lemma close_id : forall k t x,
+      (forall w l, (w, (k, l)) ∈md t -> close_loc k x (w, l) = l) ->
+      '[k | x] t = t.
+  Proof.
+    intros. unfold close.
+    now apply (kfmapd_respectful_id).
+  Qed.
+
+  (** ** Context-sensitive leaf analysis of operations *)
+  (******************************************************************************)
+
+  (** *** For [open] *)
+  (******************************************************************************)
+  Lemma ind_open_iff_eq : forall k l w u t,
+      (w, (k, l)) ∈md t '(k | u) <-> exists w1 w2 l1,
+        (w1, (k, l1)) ∈md t /\ (w2, (k, l)) ∈md open_loc k u (w1, l1) /\ w = w1 ● w2.
+  Proof.
+    intros. unfold open.
+    now rewrite (ind_kbindd_eq_iff S).
+  Qed.
+
+  Lemma ind_open_neq_iff : forall k j l w u t,
+      k <> j ->
+      (w, (k, l)) ∈md t '(j | u) <-> (w, (k, l)) ∈md t \/ exists w1 w2 l1,
+          (w1, (j, l1)) ∈md t /\ (w2, (k, l)) ∈md open_loc j u (w1, l1) /\ w = w1 ● w2.
+  Proof.
+    intros. unfold open.
+    now rewrite (ind_kbindd_neq_iff S); auto.
+  Qed.
+
+  (** *** For [close] *)
+  (******************************************************************************)
+  Lemma ind_close_iff_eq : forall k l w x t,
+      (w, (k, l)) ∈md '[k | x] t <-> exists l1,
+        (w, (k, l1)) ∈md t /\ l = close_loc k x (w, l1).
+  Proof.
+    intros. unfold close.
+    rewrite (ind_kfmapd_eq_iff S).
+    easy.
+  Qed.
+
+  Lemma ind_close_neq_iff : forall k j l w x t,
+      j <> k ->
+      (w, (k, l)) ∈md '[j | x] t <-> (w, (k, l)) ∈md t.
+  Proof.
+    intros. unfold close.
+    now rewrite (ind_kfmapd_neq_iff S).
+  Qed.
+
+  (** *** For [subst] *)
+  (******************************************************************************)
+  Lemma ind_subst_iff_eq : forall k w l u t x,
+      (w, (k, l)) ∈md t '{k | x ~> u} <-> exists w1 w2 l1,
+        (w1, (k, l1)) ∈md t /\ (w2, (k, l)) ∈md subst_loc k x u l1 /\ w = w1 ● w2.
+  Proof.
+    intros. unfold subst.
+    now rewrite (ind_kbind_eq_iff S).
+  Qed.
+
+  Lemma ind_subst_neq_iff : forall k j w l u t x,
+      k <> j ->
+      (w, (k, l)) ∈md t '{j | x ~> u} <-> (w, (k, l)) ∈md t \/ exists w1 w2 l1,
+        (w1, (j, l1)) ∈md t /\ (w2, (k, l)) ∈md subst_loc j x u l1 /\ w = w1 ● w2.
+  Proof.
+    intros. unfold subst.
+    now rewrite (ind_kbind_neq_iff S); auto.
+  Qed.
+
+  (** ** Context-agnostic leaf analysis of operations *)
+  (******************************************************************************)
+
+  (** *** For [open] *)
+  (******************************************************************************)
+  Lemma in_open_eq_iff : forall k l u t,
+      (k, l) ∈m t '(k | u) <-> exists w1 l1,
+        (w1, (k, l1)) ∈md t /\ (k, l) ∈m open_loc k u (w1, l1).
+  Proof.
+    intros. unfold open.
+    now rewrite (in_kbindd_eq_iff S).
+  Qed.
+
+  Lemma in_open_neq_iff : forall k j l u t,
+      k <> j ->
+      (k, l) ∈m t '(j | u) <-> (k, l) ∈m t \/ exists w1 l1,
+          (w1, (j, l1)) ∈md t /\ (k, l) ∈m open_loc j u (w1, l1).
+  Proof.
+    intros. unfold open.
+    now rewrite (in_kbindd_neq_iff S); auto.
+  Qed.
+
+  (** *** For [close] *)
+  (******************************************************************************)
+  Lemma in_close_eq_iff : forall k l x t,
+      (k, l) ∈m '[k | x] t <-> exists w l1,
+        (w, (k, l1)) ∈md t /\ l = close_loc k x (w, l1).
+  Proof.
+    intros. unfold close.
+    now rewrite (in_kfmapd_eq_iff S).
+  Qed.
+
+  Lemma in_close_neq_iff : forall k j l x t,
+      k <> j ->
+      (k, l) ∈m '[j | x] t <-> (k, l) ∈m t.
+  Proof.
+    intros. unfold close.
+    now rewrite (in_kfmapd_neq_iff S); auto.
+  Qed.
+
+  (** *** For [subst] *)
+  (******************************************************************************)
+  Lemma in_subst_eq_iff : forall k l u t x,
+      (k, l) ∈m t '{k | x ~> u} <-> exists l1,
+        (k, l1) ∈m t /\ (k, l) ∈m subst_loc k x u l1.
+  Proof.
+    intros. unfold subst.
+    now rewrite (in_kbind_eq_iff S).
+  Qed.
+
+  Lemma in_subst_neq_iff : forall k j l u t x,
+      j <> k ->
+      (k, l) ∈m t '{j | x ~> u} <-> (k, l) ∈m t \/ exists l1,
+          (j, l1) ∈m t /\ (k, l) ∈m subst_loc j x u l1.
+  Proof.
+    intros. unfold subst.
+    now rewrite (in_kbind_neq_iff S).
+  Qed.
+
+End operations_specifications.
+
+
+(** * Specifications for <<free>> *)
+(******************************************************************************)
+Section operations_specifications.
+
+  (** ** Characterizations for [free] and [freeset] *)
+  (******************************************************************************)
+  Section characterize_free.
+
+    Context
+      (S : Type -> Type)
+      `{DTPreModule (list K) S T (mn_op := Monoid_op_list) (mn_unit := Monoid_unit_list)}
+      `{! DTM (list K) T}.
+
+    Theorem in_free_iff : forall (k : K) (t : S leaf) (x : atom),
+        x ∈ free S k t <-> (k, Fr x) ∈m t.
+    Proof.
+      intros. unfold free. rewrite (Tealeaves.Classes.SetlikeMonad.in_bind_iff list). split.
+      - intros [l [lin xin]]. rewrite <- (in_iff_in_toklist) in lin.
+        destruct l as [a|n].
+        + cbv in xin. destruct xin as [?|[]].
+          subst. assumption.
+        + cbv in xin. destruct xin as [].
+      - intros. exists (Fr x). rewrite <- (in_iff_in_toklist).
+        split; [assumption| ].
+        cbv. now left.
+    Qed.
+
+    Corollary free_iff_freeset : forall (k : K) (t : S leaf) (x : atom),
+        x ∈ free S k t <-> x ∈@ freeset S k t.
+    Proof.
+      intros. unfold freeset. rewrite <- in_atoms_iff.
+      reflexivity.
+    Qed.
+
+  End characterize_free.
+
+  (** ** [free] variables after <<open>>/<<close>>/<<subst>> *)
+  (******************************************************************************)
+  Context
+    (S : Type -> Type)
+    `{DTPreModule (list K) S T (mn_op := Monoid_op_list) (mn_unit := Monoid_unit_list)}
+    `{! DTM (list K) T}.
+
+  (** *** After [open] *)
+  (******************************************************************************)
+  Lemma free_open_eq_iff : forall k u t x,
+      x ∈ free S k (t '(k | u)) <-> exists w l1,
+        (w, (k, l1)) ∈md t /\ x ∈ free (T k) k (open_loc k u (w, l1)).
+  Proof.
+    intros. rewrite in_free_iff.
+    setoid_rewrite in_free_iff.
+    now rewrite in_open_eq_iff.
+  Qed.
+
+  Lemma free_open_neq_iff : forall k j u t x,
+      k <> j ->
+      x ∈ free S j (t '(k | u)) <-> x ∈ free S j t \/ exists w l1,
+          (w, (k, l1)) ∈md t /\ x ∈ free (T k) j (open_loc k u (w, l1)).
+  Proof.
+    intros. rewrite 2(in_free_iff). setoid_rewrite in_free_iff.
+    now rewrite in_open_neq_iff; auto.
+  Qed.
+
+  (** *** After [close] *)
+  (******************************************************************************)
+  Lemma free_close_eq_iff : forall k t x y,
+      y ∈ free S k ('[k | x] t) <-> exists w l1,
+        (w, (k, l1)) ∈md t /\ Fr y = close_loc k x (w, l1).
+  Proof.
+    intros. rewrite (in_free_iff S).
+    now rewrite (in_close_eq_iff S).
+  Qed.
+
+  Lemma free_close_neq_iff : forall k j t x,
+      k <> j ->
+      x ∈ free S j ('[k | x] t) <-> x ∈ free S j t.
+  Proof.
+    intros. rewrite 2(in_free_iff).
+    now rewrite (in_close_neq_iff S); auto.
+  Qed.
+
+  (** *** For [subst] *)
+  (******************************************************************************)
+  Lemma free_subst_eq_iff : forall k u t x y,
+      y ∈ free S k (t '{k | x ~> u}) <-> exists l1,
+        (k, l1) ∈m t /\ y ∈ free (T k) k (subst_loc k x u l1).
+  Proof.
+    intros. rewrite (in_free_iff). setoid_rewrite (in_free_iff (T k)).
+    now rewrite (in_subst_eq_iff S).
+  Qed.
+
+  Lemma free_subst_neq_iff : forall j k u t x y,
+      k <> j ->
+      y ∈ free S j (t '{k | x ~> u}) <-> y ∈ free S j t \/ exists l1,
+        (k, l1) ∈m t /\ y ∈ free (T k) j (subst_loc k x u l1).
+  Proof.
+    intros. rewrite 2(in_free_iff). setoid_rewrite (in_free_iff (T k)).
+    now rewrite (in_subst_neq_iff); auto.
+  Qed.
+
+End operations_specifications.
 
 (** * Lemmas for local reasoning *)
 (** The following lemmas govern the behavior of the <<*_loc>> operations of
@@ -29,10 +319,9 @@ Import DTMContainer.Notations.
       <<autorewrite*>>, which only uses hints whose side conditions are
       discharged by the associated tactic. *)
 (******************************************************************************)
-
 Create HintDb tea_local.
 
-Section locally_nameless_utilities.
+Section locally_nameless_local.
 
   Context
     (S : Type -> Type)
@@ -41,7 +330,7 @@ Section locally_nameless_utilities.
 
   Implicit Types (l : leaf) (w : list K) (t : S leaf) (x : atom) (j k : K) (n : nat).
 
-  (** ** (In)equalities between leaves *)
+  (** ** Lemmas for proving (in)equalities between leaves *)
   (******************************************************************************)
   Lemma Fr_injective : forall (x y : atom),
       (Fr x = Fr y) <-> (x = y).
@@ -69,25 +358,57 @@ Section locally_nameless_utilities.
     introv. propext. discriminate. contradiction.
   Qed.
 
+  Lemma prod_K_not_iff : forall (k : K) A (x y : A),
+      ((k, x) <> (k, y)) <-> (x <> y).
+  Proof.
+    intros. split; intro hyp; contradict hyp.
+    now subst. now injection hyp.
+  Qed.
+
+  Lemma ninf_in_neq : forall k x l (t : S leaf),
+      ~ x ∈ free S k t ->
+      (k, l) ∈m t -> Fr x <> l.
+  Proof.
+    introv hyp1 hyp2.
+    rewrite in_free_iff in hyp1. destruct l.
+    - injection. intros; subst.
+      contradiction.
+    - discriminate.
+  Qed.
+
+  Lemma neq_symmetry : forall X (x y : X),
+      (x <> y) = (y <> x).
+  Proof.
+    intros. propext; intro hyp; contradict hyp; congruence.
+  Qed.
+
   (** ** [subst_loc] *)
   (******************************************************************************)
   Lemma subst_loc_eq : forall k u x,
       subst_loc k x u (Fr x) = u.
-  Proof. intros. cbn. now compare values x and x. Qed.
+  Proof.
+    intros. cbn. now compare values x and x.
+  Qed.
 
   Lemma subst_loc_neq : forall k u x y,
-      y <> x -> subst_loc k x u (Fr y) = mret T k (Fr y).
-  Proof. intros. cbn. now compare values x and y. Qed.
+      y <> x ->
+      subst_loc k x u (Fr y) = mret T k (Fr y).
+  Proof.
+    intros. cbn. now compare values x and y.
+  Qed.
 
   Lemma subst_loc_b : forall k u x n,
       subst_loc k x u (Bd n) = mret T k (Bd n).
-  Proof. reflexivity. Qed.
+  Proof.
+    reflexivity.
+  Qed.
 
   Lemma subst_loc_fr_neq : forall k u l x,
-      Fr x <> l -> subst_loc k x u l = mret T k l.
+      Fr x <> l ->
+      subst_loc k x u l = mret T k l.
   Proof.
     introv neq. unfold subst_loc.
-    destruct l as [a|?]; [compare values x and a | reflexivity ].
+    destruct l as [a|?]; [compare values x and a | reflexivity].
   Qed.
 
   Lemma subst_in_mret_eq : forall k x l u,
@@ -108,13 +429,15 @@ Section locally_nameless_utilities.
   (** ** [open_loc] *)
   (******************************************************************************)
   Lemma open_loc_lt : forall k u w n,
-      n < countk k w -> open_loc k u (w, Bd n) = mret T k (Bd n).
+      n < countk k w ->
+      open_loc k u (w, Bd n) = mret T k (Bd n).
   Proof.
     introv ineq. unfold open_loc. compare naturals n and (countk k w).
   Qed.
 
   Lemma open_loc_gt : forall k u n w,
-      n > countk k w -> open_loc k u (w, Bd n) = mret T k (Bd (n - 1)).
+      n > countk k w ->
+      open_loc k u (w, Bd n) = mret T k (Bd (n - 1)).
   Proof.
     introv ineq. unfold open_loc. compare naturals n and (countk k w).
   Qed.
@@ -131,63 +454,662 @@ Section locally_nameless_utilities.
     reflexivity.
   Qed.
 
-  (** ** [Miscellaneous utilities] *)
-  (******************************************************************************)
-  Lemma ninf_in_neq : forall k x l (t : T k leaf),
-      ~ x ∈ free (T k) k t ->
-      (k, l) ∈m t -> Fr x <> l.
-  Proof.
-    introv hyp1 hyp2.
-    rewrite in_free_iff in hyp1. destruct l.
-    - injection. intros; subst.
-      contradiction.
-    - discriminate.
-  Qed.
+End locally_nameless_local.
 
-  Lemma ninf_in_neq_t : forall k' (t : T k' leaf) k x l,
-      ~ x ∈ free (T k') k t -> (k, l) ∈m t -> Fr x <> l.
-  Proof.
-    introv hyp1 hyp2.
-    rewrite in_free_iff in hyp1. destruct l.
-    - injection. intros; subst.
-      contradiction.
-    - discriminate.
-  Qed.
-
-  Lemma neq_symmetry : forall X (x y : X),
-      (x <> y) = (y <> x).
-  Proof.
-    intros. propext; intro hyp; contradict hyp; congruence.
-  Qed.
-
-End locally_nameless_utilities.
-
+(** ** Tactics for local reasoning *)
+(******************************************************************************)
 Tactic Notation "unfold_monoid" :=
   repeat unfold monoid_op, Monoid_op_list, Monoid_op_list,
   monoid_unit, Monoid_unit_list, Monoid_unit_list in *.
 
-Tactic Notation "unfold_lia" :=
-  unfold_monoid; lia.
+Hint Rewrite @prod_K_not_iff : tea_local.
 
-Hint Rewrite @in_mret_iff @in_mret_eq_iff
+(** Rewrite rules for expressions of the form <<x ∈ mret T y>> *)
+Hint Rewrite
+     @in_mret_iff @in_mret_eq_iff
      @ind_mret_iff @ind_mret_eq_iff using typeclasses eauto : tea_local.
 
-Hint Rewrite Fr_injective Fr_injective_not_iff B_neq_Fr : tea_local.
-#[export] Hint Resolve Fr_injective_not : tea_local.
+(** Rewrite rules for simplifying expressions involving equalities between leaves *)
+Hint Rewrite
+     Fr_injective Fr_injective_not_iff B_neq_Fr : tea_local.
 
-Hint Rewrite @subst_loc_eq @subst_in_mret_eq using typeclasses eauto : tea_local.
-Hint Rewrite @subst_loc_neq @subst_loc_b @subst_loc_fr_neq @subst_in_mret_neq
-     using first [ typeclasses eauto | auto ] : tea_local.
+(** Solve goals of the form <<Fr x <> Fr y>> by using <<x <> y>> *)
+#[export] Hint Resolve
+ Fr_injective_not : tea_local.
 
-Hint Rewrite @open_loc_lt @open_loc_gt
+Hint Rewrite
+     @subst_loc_eq @subst_in_mret_eq
+     using typeclasses eauto : tea_local.
+Hint Rewrite
+     @subst_loc_neq @subst_loc_b @subst_loc_fr_neq @subst_in_mret_neq
      using first [ typeclasses eauto | auto ] : tea_local.
-Hint Rewrite @open_loc_eq @open_loc_atom using typeclasses eauto : tea_local.
+Hint Rewrite
+     @open_loc_lt @open_loc_gt
+     using first [ typeclasses eauto | auto ] : tea_local.
+Hint Rewrite
+     @open_loc_eq @open_loc_atom
+     using typeclasses eauto : tea_local.
 
 Tactic Notation "simpl_local" := (autorewrite* with tea_local).
 
-(** * Locally nameless metatheory *)
+(** * Metatheory for the <<subst>> operation *)
 (******************************************************************************)
-Section locally_nameless_metatheory.
+Section subst_metatheory.
+
+  Section fix_dtm.
+
+    Context
+      (S : Type -> Type)
+      `{DTPreModule (list K) S T (mn_op := Monoid_op_list) (mn_unit := Monoid_unit_list)}
+      `{! DTM (list K) T}.
+
+    Implicit Types
+             (k : K) (j : K)
+             (l : leaf) (p : leaf)
+             (x : atom) (t : S leaf)
+             (w : list K) (n : nat).
+
+    (** ** Leaf analysis with contexts *)
+    (******************************************************************************)
+    Lemma ind_subst_loc_iff : forall k l w j p u x,
+        (w, (j, p)) ∈md subst_loc k x u l <->
+        l <> Fr x /\ k = j /\ w = Ƶ /\ l = p \/ (* l is not replaced *)
+        l = Fr x /\ (w, (j, p)) ∈md u. (* l is replaced *)
+    Proof.
+      introv. compare l to atom x.
+      - rewrite subst_loc_eq.
+        clear; firstorder.
+      - rewrite subst_loc_neq; auto.
+        rewrite ind_mret_iff.
+        rewrite Fr_injective.
+        firstorder.
+      - rewrite subst_loc_b.
+        rewrite ind_mret_iff.
+        rewrite B_neq_Fr.
+        firstorder.
+    Qed.
+
+    Corollary ind_subst_loc_iff_eq : forall k l w p u x,
+        (w, (k, p)) ∈md subst_loc k x u l <->
+        l <> Fr x /\ w = Ƶ /\ l = p \/
+        l = Fr x /\ (w, (k, p)) ∈md u.
+    Proof.
+      introv. rewrite ind_subst_loc_iff. clear. firstorder.
+    Qed.
+
+    Corollary ind_subst_loc_iff_neq : forall k l w j p u x,
+        k <> j ->
+        (w, (j, p)) ∈md subst_loc k x u l <->
+        l = Fr x /\ (w, (j, p)) ∈md u.
+    Proof.
+      introv neq. rewrite ind_subst_loc_iff. intuition.
+    Qed.
+
+    Theorem ind_subst_iff : forall k j w t u l x,
+        (* <<l>> occurs in the result of a <<subst>> IFF *)
+        (w, j, l) ∈md t '{k | x ~> u} <->
+        (* <<l>> is an occurrence in <<t>> not of the same sort as the <<subst>> OR *)
+        k <> j /\ (w, j, l) ∈md t \/
+        (* <<l>> is an occurrence of the same sort but not an occurrence of <<x>> OR *)
+        k = j /\ (w, k, l) ∈md t /\ l <> Fr x \/
+        (* <<x>> occurs and <<l>> is the any leaf in a substituted <<u>> *)
+        exists w1 w2 : list K, (w1, k, Fr x) ∈md t /\ (w2, j, l) ∈md u /\ w = w1 ● w2.
+    Proof with auto.
+      intros. compare values k and j.
+      - rewrite (ind_subst_iff_eq S). setoid_rewrite (ind_subst_loc_iff_eq j).
+        split.
+        + intros [l' [n1 [n2 conditions]]].
+          right. destruct conditions as [c1 [[c2|c2] c3]].
+          { subst. left. destructs c2; subst.
+            rewrite monoid_id_l. auto. }
+          { subst. right. destructs c2; subst. eauto. }
+        + intros [[contra ?] | [ [? [in_t neq]] | hyp ] ].
+          { contradiction. }
+          { exists w (Ƶ : list K) l. rewrite monoid_id_l. split... }
+          { destruct hyp as [w1 [w2 ?]]. exists w1 w2 (Fr x). intuition. }
+      - rewrite (ind_subst_neq_iff S)... split.
+        + intros [? | [n1 [n2 [p [in_t in_local]]]]]...
+          rewrite (ind_subst_loc_iff_neq k) in in_local...
+          right. right. exists n1 n2. destruct in_local as [[? ?] ?]; subst...
+        + intros [[? ?] | [[? ?] | [w1 [w2 rest]]]].
+          { auto. }
+          { contradiction. }
+          { right. exists w1 w2 (Fr x). simpl_local... }
+    Qed.
+
+    Corollary ind_subst_iff_eq' : forall k w t u l x,
+        (w, k, l) ∈md t '{k | x ~> u} <->
+        (w, k, l) ∈md t /\ l <> Fr x \/
+        exists w1 w2 : list K, (w1, k, Fr x) ∈md t /\ (w2, k, l) ∈md u /\ w = w1 ● w2.
+    Proof.
+      intros. rewrite ind_subst_iff. intuition.
+    Qed.
+
+    Corollary ind_subst_iff_neq' : forall k j w t u l x,
+        k <> j ->
+        (w, j, l) ∈md t '{k | x ~> u} <->
+        (w, j, l) ∈md t \/
+        exists w1 w2 : list K, (w1, k, Fr x) ∈md t /\ (w2, j, l) ∈md u /\ w = w1 ● w2.
+    Proof.
+      intros. rewrite ind_subst_iff. intuition.
+    Qed.
+
+    (** ** Leaf analysis without contexts *)
+    (******************************************************************************)
+    Lemma in_subst_loc_iff : forall k l j p u x,
+        (j, p) ∈m subst_loc k x u l <->
+        l <> Fr x /\ k = j /\ l = p \/
+        l = Fr x /\ (j, p) ∈m u.
+    Proof.
+      introv. compare l to atom x; autorewrite* with tea_local; intuition.
+    Qed.
+
+    Corollary in_subst_loc_iff_eq : forall k l p u x,
+        (k, p) ∈m subst_loc k x u l <->
+        l <> Fr x /\ l = p \/
+        l = Fr x /\ (k, p) ∈m u.
+    Proof.
+      introv. rewrite in_subst_loc_iff; intuition.
+    Qed.
+
+    Corollary in_subst_loc_iff_neq : forall k l j p u x,
+        k <> j ->
+        (j, p) ∈m subst_loc k x u l <->
+        l = Fr x /\ (j, p) ∈m u.
+    Proof.
+      introv neq. rewrite in_subst_loc_iff. intuition.
+    Qed.
+
+    Theorem in_subst_iff : forall k j t u l x,
+        (* <<l>> occurs in the result of a <<subst>> IFF *)
+        (j, l) ∈m t '{k | x ~> u} <->
+        (* <<l>> is an occurrence in <<t>> not of the same sort as the <<subst>> OR *)
+        k <> j /\ (j, l) ∈m t \/
+        (* <<l>> is an occurrence of the same sort but not an occurrence of <<x>> OR *)
+        k = j /\ (k, l) ∈m t /\ l <> Fr x \/
+        (* <<x>> occurs and <<l>> is the any leaf in a substituted <<u>> *)
+        (k, Fr x) ∈m t /\ (j, l) ∈m u.
+    Proof with auto.
+      intros. destruct_eq_args k j.
+      - rewrite (in_subst_eq_iff S).
+        setoid_rewrite (in_subst_loc_iff_eq). split.
+        + intros [? [?  in_sub]].
+          destruct in_sub as [[? heq] | [heq ?]]; subst...
+        + intros [[contra ?] | [ [? [in_t neq]] | ? ] ].
+          { contradiction.  }
+          { exists l... }
+          { exists (Fr x). intuition. }
+      - rewrite (in_subst_neq_iff S); auto. split.
+        + intros [? | [p [in_t in_local]] ]; auto.
+          rewrite in_subst_loc_iff_neq in in_local; auto.
+          destruct in_local as [? ?]; subst. auto.
+        + intros [[? ?] | [[? ?] | ?]].
+          { auto. }
+          { contradiction. }
+          { right. exists (Fr x). simpl_local... }
+    Qed.
+
+    Corollary in_subst_iff_eq : forall k t u l x,
+        (k, l) ∈m t '{k | x ~> u} <->
+        (k, l) ∈m t /\ l <> Fr x \/
+        (k, Fr x) ∈m t /\ (k, l) ∈m u.
+    Proof with auto.
+      intros. rewrite in_subst_iff. intuition.
+    Qed.
+
+    Corollary in_subst_iff_neq : forall k j t u l x,
+        k <> j ->
+        (j, l) ∈m t '{k | x ~> u} <->
+        (j, l) ∈m t \/
+        (k, Fr x) ∈m t /\ (j, l) ∈m u.
+    Proof with auto.
+      intros. rewrite in_subst_iff. intuition.
+    Qed.
+
+    (** ** Free variables after substitution *)
+    (******************************************************************************)
+    Corollary in_free_subst_iff_eq : forall t k u x y,
+        y ∈ free S k (t '{k | x ~> u}) <->
+        y ∈ free S k t /\ y <> x \/ x ∈ free S k t /\ y ∈ free (T k) k u.
+    Proof.
+      intros. repeat rewrite (in_free_iff).
+      rewrite in_subst_iff_eq. now simpl_local.
+    Qed.
+
+    Corollary in_freeset_subst_iff_eq : forall t k u x y,
+        y ∈@ freeset S k (t '{k | x ~> u}) <->
+        y ∈@ freeset S k t /\ y <> x \/
+        x ∈@ freeset S k t /\ y ∈@ freeset (T k) k u.
+    Proof.
+      intros. repeat rewrite <- (free_iff_freeset).
+      apply in_free_subst_iff_eq.
+    Qed.
+
+    Corollary in_free_subst_iff_neq : forall t k j u x y,
+        k <> j ->
+        y ∈ free S j (t '{k | x ~> u}) <->
+        y ∈ free S j t \/ x ∈ free S k t /\ y ∈ free (T k) j u.
+    Proof.
+      intros. repeat rewrite (in_free_iff).
+      rewrite in_subst_iff_neq; auto. reflexivity.
+    Qed.
+
+    Corollary in_freeset_subst_iff_neq : forall t k j u x y,
+        k <> j ->
+        y ∈@ freeset S j (t '{k | x ~> u}) <->
+        y ∈@ freeset S j t \/
+        x ∈@ freeset S k t /\ y ∈@ freeset (T k) j u.
+    Proof.
+      intros. repeat rewrite <- (free_iff_freeset).
+      auto using in_free_subst_iff_neq.
+    Qed.
+
+    (** ** Upper and lower bounds for leaves after substitution *)
+    (******************************************************************************)
+    Corollary in_subst_upper : forall k j t u l x,
+        (j, l) ∈m t '{k | x ~> u} ->
+        (j, l) ∈m t /\ (j, l) <> (k, Fr x) \/ (j, l) ∈m u.
+    Proof with auto.
+      introv hin. rewrite in_subst_iff in hin.
+      destruct hin as [[hyp1 hyp2] | [hyp | hyp] ].
+      - left. split; [assumption |]. injection...
+      - destructs hyp. subst. left.
+        split; [assumption |]. injection...
+      - intuition.
+    Qed.
+
+    Corollary in_subst_upper_eq : forall k t u l x,
+        (k, l) ∈m t '{k | x ~> u} ->
+        (k, l) ∈m t /\ l <> Fr x \/ (k, l) ∈m u.
+    Proof.
+      introv hyp. apply in_subst_upper in hyp.
+      autorewrite* with tea_local in hyp.
+      intuition.
+    Qed.
+
+    Corollary in_subst_upper_neq : forall k j t u l x,
+        k <> j ->
+        (j, l) ∈m t '{k | x ~> u} ->
+        (j, l) ∈m t \/ (j, l) ∈m u.
+    Proof.
+      introv neq hyp. apply in_subst_upper in hyp.
+      intuition.
+    Qed.
+
+    Corollary in_free_subst_upper : forall k j t u x y,
+        y ∈ free S j (t '{k | x ~> u}) ->
+        (y ∈ free S j t /\ j <> k) \/ (y ∈ free S k t /\ y <> x /\ k = j) \/ y ∈ free (T k) j u.
+    Proof.
+      setoid_rewrite (in_free_iff). introv hyp.
+      apply in_subst_upper in hyp.
+      destruct hyp as [hyp | hyp].
+      - destruct hyp. compare values j and k.
+        + right. left. splits; auto.
+          intro contra; subst; contradiction.
+        + auto.
+      - eauto using in_subst_upper.
+    Qed.
+
+    Corollary in_free_subst_upper_eq : forall k t u x y,
+        y ∈ free S k (t '{k | x ~> u}) ->
+        (y ∈ free S k t /\ y <> x) \/ y ∈ free (T k) k u.
+    Proof.
+      introv hyp. apply in_free_subst_upper in hyp.
+      intuition.
+    Qed.
+
+    Corollary in_free_subst_upper_neq : forall k j t u x y,
+        k <> j ->
+        y ∈ free S j (t '{k | x ~> u}) ->
+        y ∈ free S j t \/ y ∈ free (T k) j u.
+    Proof.
+      introv neq hyp. apply in_free_subst_upper in hyp.
+      intuition.
+    Qed.
+
+    Corollary freeset_subst_upper : forall k j t u x y,
+        y ∈@ freeset S j (t '{k | x ~> u}) ->
+        k = j /\ y ∈@ (freeset S k t \\ {{x}} ∪ freeset (T k) j u) \/
+        k <> j /\ y ∈@ (freeset S j t ∪ freeset (T k) j u).
+    Proof.
+      setoid_rewrite AtomSet.union_spec.
+      setoid_rewrite AtomSet.diff_spec.
+      setoid_rewrite <- free_iff_freeset.
+      introv hyp. apply in_free_subst_upper in hyp.
+      compare values j and k.
+      + left. destruct hyp as [hyp | [hyp | hyp]].
+        { split; auto. intuition. }
+        { split; auto. left. split. intuition. fsetdec. }
+        { split; auto. }
+      + right. split; auto. destruct hyp as [hyp | [hyp | hyp]].
+        { intuition. }
+        { intuition. }
+        { intuition. }
+    Qed.
+
+    Corollary freeset_subst_upper_eq : forall k t u x,
+        freeset S k (t '{k | x ~> u}) ⊆
+                (freeset S k t \\ {{x}} ∪ freeset (T k) k u).
+    Proof.
+      intros. intros a hyp. apply freeset_subst_upper in hyp.
+      intuition.
+    Qed.
+
+    Corollary freeset_subst_upper_neq : forall k j t u x,
+        k <> j ->
+        freeset S j (t '{k | x ~> u}) ⊆
+                (freeset S j t ∪ freeset (T k) j u).
+    Proof.
+      intros. intros a hyp. apply freeset_subst_upper in hyp.
+      intuition.
+    Qed.
+
+    Corollary in_subst_lower_eq : forall t k u l x,
+        (k, l) ∈m t /\ l <> Fr x ->
+        (k, l) ∈m t '{k | x ~> u}.
+    Proof with auto.
+      intros; rewrite in_subst_iff...
+    Qed.
+
+    Corollary in_subst_lower_neq : forall t k j u l x,
+        k <> j ->
+        (j, l) ∈m t ->
+        (j, l) ∈m t '{k | x ~> u}.
+    Proof with auto.
+      intros; rewrite in_subst_iff...
+    Qed.
+
+    Corollary in_free_subst_lower_eq : forall t k (u : T k leaf) x y,
+        y ∈ free S k t /\ y <> x ->
+        y ∈ free S k (t '{k | x ~> u}).
+    Proof.
+      setoid_rewrite (in_free_iff). intros.
+      apply in_subst_lower_eq. now simpl_local.
+    Qed.
+
+    Corollary in_free_subst_lower_neq : forall t k j u x y,
+        k <> j ->
+        y ∈ free S j t ->
+        y ∈ free S j (t '{k | x ~> u}).
+    Proof.
+      setoid_rewrite (in_free_iff). intros.
+      now apply in_subst_lower_neq.
+    Qed.
+
+    Corollary freeset_subst_lower_eq : forall t k (u : T k leaf) x,
+        freeset S k t \\ {{ x }} ⊆ freeset S k (t '{k | x ~> u}).
+    Proof.
+      introv. intro a. rewrite AtomSet.diff_spec.
+      do 2 rewrite <- (free_iff_freeset).
+      intros [? ?]. apply in_free_subst_lower_eq.
+      intuition.
+    Qed.
+
+    Corollary freeset_subst_lower_eq_alt : forall t k (u : T k leaf) x,
+        freeset S k t ⊆ freeset S k (t '{k | x ~> u}) ∪ {{ x }}.
+    Proof.
+      introv. intro a. rewrite AtomSet.union_spec.
+      do 2 rewrite <- (free_iff_freeset).
+      destruct_eq_args a x.
+      - right. fsetdec.
+      - left. auto using in_free_subst_lower_eq.
+    Qed.
+
+    Corollary freeset_subst_lower_neq : forall t k j u x,
+        k <> j ->
+        freeset S j t ⊆
+                freeset S j (t '{k | x ~> u}).
+    Proof.
+      introv neq. intro a.
+      do 2 rewrite <- (free_iff_freeset).
+      now apply in_free_subst_lower_neq.
+    Qed.
+
+    (** ** Substitution of fresh variables *)
+    (******************************************************************************)
+    Theorem subst_fresh : forall t k x u,
+        ~ x ∈ free S k t ->
+        t '{k | x ~> u} = t.
+    Proof.
+      intros. apply (subst_id S). intros.
+      assert (Fr x <> l).
+      eapply (ninf_in_neq S); eauto.
+      now simpl_local.
+    Qed.
+
+    Corollary subst_fresh_set : forall t k x u,
+        ~ x ∈@ freeset S k t ->
+        t '{k | x ~> u} = t.
+    Proof.
+      setoid_rewrite <- free_iff_freeset. apply subst_fresh.
+    Qed.
+
+    Theorem free_subst_fresh : forall t k j u x,
+        ~ x ∈ free S k t ->
+        free S j (t '{k | x ~> u}) = free S j t.
+    Proof with auto.
+      introv fresh. replace (t '{k | x ~> u}) with t...
+      rewrite subst_fresh...
+    Qed.
+
+    Corollary free_subst_fresh_eq : forall t k u x,
+        ~ x ∈ free S k t ->
+        free S k (t '{k | x ~> u}) = free S k t.
+    Proof.
+      introv fresh. replace (t '{k | x ~> u}) with t; auto.
+      now rewrite subst_fresh.
+    Qed.
+
+    Corollary freeset_subst_fresh : forall t k j u x,
+        ~ x ∈@ freeset S k t ->
+        freeset S j (t '{k | x ~> u}) [=] freeset S j t.
+    Proof.
+      introv fresh. intro y.
+      rewrite <- ?(free_iff_freeset) in *.
+      now rewrite free_subst_fresh.
+    Qed.
+
+    Corollary freeset_subst_fresh_eq : forall t k u x,
+        ~ x ∈@ freeset S k t ->
+        freeset S k (t '{k | x ~> u}) [=] freeset S k t.
+    Proof.
+      intros. apply freeset_subst_fresh; auto.
+    Qed.
+
+  End fix_dtm.
+
+  (** ** Composing substitutions *)
+  (******************************************************************************)
+  Section fix_dtm.
+
+    Context
+      (S : Type -> Type)
+      `{DTPreModule (list K) S T (mn_op := Monoid_op_list) (mn_unit := Monoid_unit_list)}
+      `{! DTM (list K) T}.
+
+    Implicit Types
+             (k : K) (j : K)
+             (l : leaf) (p : leaf)
+             (x : atom) (t : S leaf)
+             (w : list K) (n : nat).
+
+    Lemma subst_subst_neq_loc : forall j k1 k2 (u1 : T k1 leaf) (u2 : T k2 leaf) (x1 x2 : atom),
+        k1 <> k2 ->
+        ~ x1 ∈ free (T k2) k1 u2 ->
+        subst (T j) k2 x2 u2 ∘ btg T k1 (subst_loc k1 x1 u1) j =
+        subst (T j) k1 x1 (subst (T k1) k2 x2 u2 u1) ∘ btg T k2 (subst_loc k2 x2 u2) j.
+    Proof with easy.
+      intros. ext l. unfold compose. compare j to both of { k1 k2 }.
+      - do 2 simpl_tgt_fallback.
+        simpl_local.
+        compare l to atom x1.
+        + rewrite 2(subst_loc_eq)...
+        + rewrite subst_loc_neq; auto. now simpl_local.
+        + rewrite subst_loc_b. now simpl_local.
+      - simpl_tgt. simpl_local. compare l to atom x2.
+        + simpl_local. rewrite (subst_fresh (T k2))...
+        + simpl_local...
+        + simpl_local...
+      - simpl_tgt_fallback. now do 2 (rewrite subst_in_mret_neq; auto).
+    Qed.
+
+    Theorem subst_subst_neq : forall k1 k2 u1 u2 t (x1 x2 : atom),
+        k1 <> k2 ->
+        ~ x1 ∈ free (T k2) k1 u2 ->
+        t '{k1 | x1 ~> u1} '{k2 | x2 ~> u2} =
+        t '{k2 | x2 ~> u2} '{k1 | x1 ~> u1 '{k2 | x2 ~> u2} }.
+    Proof.
+      intros. unfold subst.
+      compose near t on left.
+      compose near t on right.
+      unfold kbind. rewrite 2(mbind_mbind S).
+      fequal. ext j. now apply subst_subst_neq_loc.
+    Qed.
+
+    Lemma subst_subst_eq_local : forall k u1 u2 x1 x2,
+        ~ x1 ∈ free (T k) k u2 ->
+        x1 <> x2 ->
+        subst (T k) k x2 u2 ∘ subst_loc k x1 u1 =
+        subst (T k) k x1 (subst (T k) k x2 u2 u1) ∘ subst_loc k x2 u2.
+    Proof with auto.
+      intros. ext l. unfold compose. compare l to atom x1.
+      - rewrite subst_loc_eq, subst_loc_neq,
+        subst_in_mret_eq, subst_loc_eq...
+      - rewrite subst_loc_neq...
+        compare values x2 and a.
+        + rewrite subst_in_mret_eq, subst_loc_eq, (subst_fresh (T k))...
+        + rewrite subst_loc_neq, 2(subst_in_mret_eq), 2(subst_loc_neq)...
+      - rewrite 2(subst_loc_b), 2(subst_in_mret_eq), 2(subst_loc_b)...
+    Qed.
+
+    Theorem subst_subst_eq : forall k u1 u2 t x1 x2,
+        ~ x1 ∈ free (T k) k u2 ->
+        x1 <> x2 ->
+        t '{k | x1 ~> u1} '{k | x2 ~> u2} =
+        t '{k | x2 ~> u2} '{k | x1 ~> u1 '{k | x2 ~> u2} }.
+    Proof with auto.
+      intros. unfold subst.
+      compose near t.
+      rewrite 2(kbind_kbind S).
+      fequal. now apply subst_subst_eq_local.
+    Qed.
+
+    (** ** Commuting two substitutions *)
+    (******************************************************************************)
+    Corollary subst_subst_comm_eq : forall k u1 u2 t x1 x2,
+        x1 <> x2 ->
+        ~ x1 ∈ free (T k) k u2 ->
+        ~ x2 ∈ free (T k) k u1 ->
+        t '{k | x1 ~> u1} '{k | x2 ~> u2} =
+        t '{k | x2 ~> u2} '{k | x1 ~> u1}.
+    Proof.
+      intros. rewrite subst_subst_eq; auto.
+      rewrite (subst_fresh (T k)); auto.
+    Qed.
+
+    Corollary subst_subst_comm_neq : forall k1 k2 u1 u2 t x1 x2,
+        k1 <> k2 ->
+        ~ x1 ∈ free (T k2) k1 u2 ->
+        ~ x2 ∈ free (T k1) k2 u1 ->
+        t '{k1 | x1 ~> u1} '{k2 | x2 ~> u2} =
+        t '{k2 | x2 ~> u2} '{k1 | x1 ~> u1}.
+    Proof.
+      intros. rewrite subst_subst_neq; auto.
+      rewrite (subst_fresh (T k1)); auto.
+    Qed.
+
+    (** ** Local closure is preserved by substitution *)
+    (******************************************************************************)
+    Theorem subst_lc_eq : forall k u t x,
+        locally_closed S k t ->
+        locally_closed (T k) k u ->
+        locally_closed S k (subst S k x u t).
+    Proof.
+      unfold locally_closed. introv lct lcu hin.
+      rewrite (ind_subst_iff_eq' S) in hin.
+      destruct hin as [[? ?] | [n1 [n2 [h1 [h2 h3]]]]].
+      - auto.
+      - subst. specialize (lcu n2 l h2).
+        unfold is_bound_or_free in *.
+        destruct l; auto. unfold_monoid.
+        rewrite countk_app. lia.
+    Qed.
+
+    Theorem subst_lc_neq : forall k j u t x,
+        k <> j ->
+        locally_closed S j t ->
+        locally_closed (T k) j u ->
+        locally_closed S j (subst S k x u t).
+    Proof.
+      unfold locally_closed. introv neq lct lcu hin.
+      rewrite (ind_subst_iff_neq' S) in hin; auto.
+      destruct hin as [? | [n1 [n2 [h1 [h2 h3]]]]].
+      - auto.
+      - subst. specialize (lcu n2 l h2).
+        unfold is_bound_or_free in *.
+        destruct l; auto. unfold_monoid.
+        rewrite countk_app. lia.
+    Qed.
+
+    (** ** Decompose substitution into closing/opening *)
+    (******************************************************************************)
+    Lemma subst_spec_local : forall k u w l x,
+        subst_loc k x u l =
+        open_loc k u (w, (close_loc k x) (w, l)).
+    Proof.
+      introv. compare l to atom x; autorewrite* with tea_local.
+      - cbn. compare values x and x. unfold id.
+        compare naturals (countk k w) and (countk k w).
+      - cbn. compare values x and a. (* todo fix fragile names *)
+      - cbn. unfold id. compare naturals n and (countk k w).
+        compare naturals (Datatypes.S (countk k w)) and (countk k w).
+        now compare naturals (Datatypes.S n) and (countk k w).
+    Qed.
+
+    Theorem subst_spec : forall k x u t,
+        t '{k | x ~> u} = ('[k | x] t) '(k | u).
+    Proof.
+      intros. compose near t on right.
+      unfold open, close, subst.
+      rewrite (kbindd_kfmapd S).
+      symmetry. apply (kbindd_respectful_kbind k).
+      symmetry. apply subst_spec_local.
+    Qed.
+
+    (** ** Substitution when <<u>> is a leaf **)
+    (******************************************************************************)
+    Definition subst_loc_leaf k x (u : leaf) : leaf -> leaf :=
+      fun l => match l with
+            | Fr y => if x == y then u else Fr y
+            | Bd n => Bd n
+            end.
+
+    Theorem subst_by_leaf_spec : forall k x l,
+        subst S k x (mret T k l) = kfmap S k (subst_loc_leaf k x l).
+    Proof.
+      intros. unfold subst. ext t.
+      apply kbind_respectful_kfmap.
+      intros l' Hin. destruct l'.
+      - cbn. compare values x and a.
+      - reflexivity.
+    Qed.
+
+    (** ** Substitution by the same variable is the identity *)
+    (******************************************************************************)
+    Theorem subst_same : forall t k x,
+        t '{k | x ~> mret T k (Fr x)} = t.
+    Proof.
+      intros. apply (subst_id S).
+      intros. compare l to atom x; now simpl_local.
+    Qed.
+
+  End fix_dtm.
+
+End subst_metatheory.
+
+(** ** Metatheory for <<close>> *)
+(******************************************************************************)
+Section close_metatheory.
 
   Context
     (S : Type -> Type)
@@ -200,624 +1122,8 @@ Section locally_nameless_metatheory.
            (x : atom) (t : S leaf)
            (w : list K) (n : nat).
 
-  (** ** Leaf analysis: substitution with contexts *)
-  (******************************************************************************)
-  Lemma ind_subst_loc_iff : forall k l w j p u x,
-      (w, (j, p)) ∈md subst_loc k x u l <->
-      l <> Fr x /\ k = j /\ w = Ƶ /\ l = p \/ (* l is not replaced *)
-      l = Fr x /\ (w, (j, p)) ∈md u. (* l is replaced *)
-  Proof.
-    introv. compare l to atom x.
-    - rewrite subst_loc_eq.
-      clear; firstorder.
-    - rewrite subst_loc_neq; auto.
-      rewrite ind_mret_iff.
-      rewrite Fr_injective.
-      firstorder.
-    - rewrite subst_loc_b.
-      rewrite ind_mret_iff.
-      rewrite B_neq_Fr.
-      firstorder.
-  Qed.
-
-  Corollary ind_subst_loc_iff_eq : forall k l w p u x,
-      (w, (k, p)) ∈md subst_loc k x u l <->
-      l <> Fr x /\ w = Ƶ /\ l = p \/
-      l = Fr x /\ (w, (k, p)) ∈md u.
-  Proof.
-    introv. rewrite ind_subst_loc_iff. clear. firstorder.
-  Qed.
-
-  Corollary ind_subst_loc_iff_neq : forall k l w j p u x,
-      k <> j ->
-      (w, (j, p)) ∈md subst_loc k x u l <->
-      l = Fr x /\ (w, (j, p)) ∈md u.
-  Proof.
-    introv neq. rewrite ind_subst_loc_iff. intuition.
-  Qed.
-
-  Theorem ind_subst_iff : forall k j w t u l x,
-      (* <<l>> occurs in the result of a <<subst>> IFF *)
-      (w, j, l) ∈md t '{k | x ~> u} <->
-      (* <<l>> is an occurrence in <<t>> not of the same sort as the <<subst>> OR *)
-      k <> j /\ (w, j, l) ∈md t \/
-      (* <<l>> is an occurrence of the same sort but not an occurrence of <<x>> OR *)
-      k = j /\ (w, k, l) ∈md t /\ l <> Fr x \/
-      (* <<x>> occurs and <<l>> is the any leaf in a substituted <<u>> *)
-      exists w1 w2 : list K, (w1, k, Fr x) ∈md t /\ (w2, j, l) ∈md u /\ w = w1 ● w2.
-  Proof with auto.
-    intros. compare values k and j.
-    - rewrite (ind_subst_iff_eq S). setoid_rewrite (ind_subst_loc_iff_eq j).
-      split.
-      + intros [l' [n1 [n2 conditions]]].
-        right. destruct conditions as [c1 [[c2|c2] c3]].
-        { subst. left. destructs c2; subst.
-          rewrite monoid_id_l. auto. }
-        { subst. right. destructs c2; subst. eauto. }
-      + intros [[contra ?] | [ [? [in_t neq]] | hyp ] ].
-        { contradiction. }
-        { exists w (Ƶ : list K) l. rewrite monoid_id_l. split... }
-        { destruct hyp as [w1 [w2 ?]]. exists w1 w2 (Fr x). intuition. }
-    - rewrite (ind_subst_neq_iff S)... split.
-      + intros [? | [n1 [n2 [p [in_t in_local]]]]]...
-        rewrite (ind_subst_loc_iff_neq k) in in_local...
-        right. right. exists n1 n2. destruct in_local as [[? ?] ?]; subst...
-      + intros [[? ?] | [[? ?] | [w1 [w2 rest]]]].
-        { auto. }
-        { contradiction. }
-        { right. exists w1 w2 (Fr x). simpl_local... }
-  Qed.
-
-  Corollary ind_subst_iff_eq : forall k w t u l x,
-      (w, k, l) ∈md t '{k | x ~> u} <->
-      (w, k, l) ∈md t /\ l <> Fr x \/
-      exists w1 w2 : list K, (w1, k, Fr x) ∈md t /\ (w2, k, l) ∈md u /\ w = w1 ● w2.
-  Proof.
-    intros. rewrite ind_subst_iff. intuition.
-  Qed.
-
-  Corollary ind_subst_iff_neq : forall k j w t u l x,
-      k <> j ->
-      (w, j, l) ∈md t '{k | x ~> u} <->
-      (w, j, l) ∈md t \/
-      exists w1 w2 : list K, (w1, k, Fr x) ∈md t /\ (w2, j, l) ∈md u /\ w = w1 ● w2.
-  Proof.
-    intros. rewrite ind_subst_iff. intuition.
-  Qed.
-
-  (** ** Leaf analysis: substitution without contexts *)
-  Lemma in_subst_loc_iff : forall k l j p u x,
-      (j, p) ∈m subst_loc k x u l <->
-      l <> Fr x /\ k = j /\ l = p \/
-      l = Fr x /\ (j, p) ∈m u.
-  Proof.
-    introv. compare l to atom x; autorewrite* with tea_local; intuition.
-  Qed.
-
-  Corollary in_subst_loc_iff_eq : forall k l p u x,
-      (k, p) ∈m subst_loc k x u l <->
-      l <> Fr x /\ l = p \/
-      l = Fr x /\ (k, p) ∈m u.
-  Proof.
-    introv. rewrite in_subst_loc_iff; intuition.
-  Qed.
-
-  Corollary in_subst_loc_iff_neq : forall k l j p u x,
-      k <> j ->
-      (j, p) ∈m subst_loc k x u l <->
-      l = Fr x /\ (j, p) ∈m u.
-  Proof.
-    introv neq. rewrite in_subst_loc_iff. intuition.
-  Qed.
-
-  Theorem in_subst_iff : forall k j t u l x,
-      (* <<l>> occurs in the result of a <<subst>> IFF *)
-      (j, l) ∈m t '{k | x ~> u} <->
-      (* <<l>> is an occurrence in <<t>> not of the same sort as the <<subst>> OR *)
-      k <> j /\ (j, l) ∈m t \/
-      (* <<l>> is an occurrence of the same sort but not an occurrence of <<x>> OR *)
-      k = j /\ (k, l) ∈m t /\ l <> Fr x \/
-      (* <<x>> occurs and <<l>> is the any leaf in a substituted <<u>> *)
-      (k, Fr x) ∈m t /\ (j, l) ∈m u.
-  Proof with auto.
-    intros. destruct_eq_args k j.
-    - rewrite (in_subst_eq_iff S).
-      setoid_rewrite (in_subst_loc_iff_eq). split.
-      + intros [? [?  in_sub]].
-        destruct in_sub as [[? heq] | [heq ?]]; subst...
-      + intros [[contra ?] | [ [? [in_t neq]] | ? ] ].
-        { contradiction.  }
-        { exists l... }
-        { exists (Fr x). intuition. }
-    - rewrite (in_subst_neq_iff S); auto. split.
-      + intros [? | [p [in_t in_local]] ]; auto.
-        rewrite in_subst_loc_iff_neq in in_local; auto.
-        destruct in_local as [? ?]; subst. auto.
-      + intros [[? ?] | [[? ?] | ?]].
-        { auto. }
-        { contradiction. }
-        { right. exists (Fr x). simpl_local... }
-  Qed.
-
-  Corollary in_subst_iff_eq : forall k t u l x,
-      (k, l) ∈m t '{k | x ~> u} <->
-      (k, l) ∈m t /\ l <> Fr x \/
-      (k, Fr x) ∈m t /\ (k, l) ∈m u.
-  Proof with auto.
-    intros. rewrite in_subst_iff. intuition.
-  Qed.
-
-  Corollary in_subst_iff_neq : forall k j t u l x,
-      k <> j ->
-      (j, l) ∈m t '{k | x ~> u} <->
-      (j, l) ∈m t \/
-      (k, Fr x) ∈m t /\ (j, l) ∈m u.
-  Proof with auto.
-    intros. rewrite in_subst_iff. intuition.
-  Qed.
-
-  (** ** Free variables after substitution *)
-    (* TODO : We can give this one an exact characterization without ∈ *)
-  Corollary in_free_subst_iff_eq : forall t k u x y,
-      y ∈ free S k (t '{k | x ~> u}) <->
-      y ∈ free S k t /\ y <> x \/ x ∈ free S k t /\ y ∈ free (T k) k u.
-  Proof.
-    intros. repeat rewrite (in_free_iff).
-    rewrite in_subst_iff_eq. now simpl_local.
-  Qed.
-
-  Corollary in_freeset_subst_iff_eq : forall t k u x y,
-      y ∈@ freeset S k (t '{k | x ~> u}) <->
-      y ∈@ freeset S k t /\ y <> x \/
-      x ∈@ freeset S k t /\ y ∈@ freeset (T k) k u.
-  Proof.
-    intros. repeat rewrite <- (free_iff_freeset).
-    apply in_free_subst_iff_eq.
-  Qed.
-
-  Corollary in_free_subst_iff_neq : forall t k j u x y,
-      k <> j ->
-      y ∈ free S j (t '{k | x ~> u}) <->
-      y ∈ free S j t \/ x ∈ free S k t /\ y ∈ free (T k) j u.
-  Proof.
-    intros. repeat rewrite (in_free_iff).
-    rewrite in_subst_iff_neq; auto. reflexivity.
-  Qed.
-
-  Corollary in_freeset_subst_iff_neq : forall t k j u x y,
-      k <> j ->
-      y ∈@ freeset S j (t '{k | x ~> u}) <->
-      y ∈@ freeset S j t \/
-      x ∈@ freeset S k t /\ y ∈@ freeset (T k) j u.
-  Proof.
-    intros. repeat rewrite <- (free_iff_freeset).
-    auto using in_free_subst_iff_neq.
-  Qed.
-
-  (** ** Upper and lower bounds for leaves after substitution *)
-  Corollary in_subst_upper : forall k j t u l x,
-      (j, l) ∈m t '{k | x ~> u} ->
-      (j, l) ∈m t /\ (j, l) <> (k, Fr x) \/ (j, l) ∈m u.
-  Proof with auto.
-    introv hin. rewrite in_subst_iff in hin.
-    destruct hin as [[hyp1 hyp2] | [hyp | hyp] ].
-    - left. split; [assumption |]. injection...
-    - destructs hyp. subst. left.
-      split; [assumption |]. injection...
-    - intuition.
-  Qed.
-
-  Lemma prod_K_not_iff : forall (k : K) A (x y : A),
-      ((k, x) <> (k, y)) <-> (x <> y).
-  Proof.
-    intros. split; intro hyp; contradict hyp.
-    now subst. now injection hyp.
-  Qed.
-
-  Hint Rewrite prod_K_not_iff : tea_local.
-
-  Corollary in_subst_upper_eq : forall k t u l x,
-      (k, l) ∈m t '{k | x ~> u} ->
-      (k, l) ∈m t /\ l <> Fr x \/ (k, l) ∈m u.
-  Proof.
-    introv hyp. apply in_subst_upper in hyp.
-    autorewrite* with tea_local in hyp.
-    intuition.
-  Qed.
-
-  Corollary in_subst_upper_neq : forall k j t u l x,
-      k <> j ->
-      (j, l) ∈m t '{k | x ~> u} ->
-      (j, l) ∈m t \/ (j, l) ∈m u.
-  Proof.
-    introv neq hyp. apply in_subst_upper in hyp.
-    intuition.
-  Qed.
-
-  Corollary in_free_subst_upper : forall k j t u x y,
-      y ∈ free S j (t '{k | x ~> u}) ->
-      (y ∈ free S j t /\ j <> k) \/ (y ∈ free S k t /\ y <> x /\ k = j) \/ y ∈ free (T k) j u.
-  Proof.
-    setoid_rewrite (in_free_iff). introv hyp.
-    apply in_subst_upper in hyp.
-    destruct hyp as [hyp | hyp].
-    - destruct hyp. compare values j and k.
-      + right. left. splits; auto.
-        intro contra; subst; contradiction.
-      + auto.
-    - eauto using in_subst_upper.
-  Qed.
-
-  Corollary in_free_subst_upper_eq : forall k t u x y,
-      y ∈ free S k (t '{k | x ~> u}) ->
-      (y ∈ free S k t /\ y <> x) \/ y ∈ free (T k) k u.
-  Proof.
-    introv hyp. apply in_free_subst_upper in hyp.
-    intuition.
-  Qed.
-
-  Corollary in_free_subst_upper_neq : forall k j t u x y,
-      k <> j ->
-      y ∈ free S j (t '{k | x ~> u}) ->
-      y ∈ free S j t \/ y ∈ free (T k) j u.
-  Proof.
-    introv neq hyp. apply in_free_subst_upper in hyp.
-    intuition.
-  Qed.
-
-  Corollary freeset_subst_upper : forall k j t u x y,
-      y ∈@ freeset S j (t '{k | x ~> u}) ->
-      k = j /\ y ∈@ (freeset S k t \\ {{x}} ∪ freeset (T k) j u) \/
-      k <> j /\ y ∈@ (freeset S j t ∪ freeset (T k) j u).
-  Proof.
-    setoid_rewrite AtomSet.union_spec.
-    setoid_rewrite AtomSet.diff_spec.
-    setoid_rewrite <- free_iff_freeset.
-    introv hyp. apply in_free_subst_upper in hyp.
-    compare values j and k.
-    + left. destruct hyp as [hyp | [hyp | hyp]].
-      { split; auto. intuition. }
-      { split; auto. left. split. intuition. fsetdec. }
-      { split; auto. }
-    + right. split; auto. destruct hyp as [hyp | [hyp | hyp]].
-      { intuition. }
-      { intuition. }
-      { intuition. }
-  Qed.
-
-  Corollary freeset_subst_upper_eq : forall k t u x,
-      freeset S k (t '{k | x ~> u}) ⊆
-              (freeset S k t \\ {{x}} ∪ freeset (T k) k u).
-  Proof.
-    intros. intros a hyp. apply freeset_subst_upper in hyp.
-    intuition.
-  Qed.
-
-  Corollary freeset_subst_upper_neq : forall k j t u x,
-      k <> j ->
-      freeset S j (t '{k | x ~> u}) ⊆
-              (freeset S j t ∪ freeset (T k) j u).
-  Proof.
-    intros. intros a hyp. apply freeset_subst_upper in hyp.
-    intuition.
-  Qed.
-
-  Corollary in_subst_lower_eq : forall t k u l x,
-      (k, l) ∈m t /\ l <> Fr x ->
-      (k, l) ∈m t '{k | x ~> u}.
-  Proof with auto.
-    intros; rewrite in_subst_iff...
-  Qed.
-
-  Corollary in_subst_lower_neq : forall t k j u l x,
-      k <> j ->
-      (j, l) ∈m t ->
-      (j, l) ∈m t '{k | x ~> u}.
-  Proof with auto.
-    intros; rewrite in_subst_iff...
-  Qed.
-
-  Corollary in_free_subst_lower_eq : forall t k (u : T k leaf) x y,
-      y ∈ free S k t /\ y <> x ->
-      y ∈ free S k (t '{k | x ~> u}).
-  Proof.
-    setoid_rewrite (in_free_iff). intros.
-    apply in_subst_lower_eq. now simpl_local.
-  Qed.
-
-  Corollary in_free_subst_lower_neq : forall t k j u x y,
-      k <> j ->
-      y ∈ free S j t ->
-      y ∈ free S j (t '{k | x ~> u}).
-  Proof.
-    setoid_rewrite (in_free_iff). intros.
-    now apply in_subst_lower_neq.
-  Qed.
-
-  Corollary freeset_subst_lower_eq : forall t k (u : T k leaf) x,
-      freeset S k t \\ {{ x }} ⊆ freeset S k (t '{k | x ~> u}).
-  Proof.
-    introv. intro a. rewrite AtomSet.diff_spec.
-    do 2 rewrite <- (free_iff_freeset).
-    intros [? ?]. apply in_free_subst_lower_eq.
-    intuition.
-  Qed.
-
-  Corollary freeset_subst_lower_eq_alt : forall t k (u : T k leaf) x,
-      freeset S k t ⊆ freeset S k (t '{k | x ~> u}) ∪ {{ x }}.
-  Proof.
-    introv. intro a. rewrite AtomSet.union_spec.
-    do 2 rewrite <- (free_iff_freeset).
-   destruct_eq_args a x.
-    - right. fsetdec.
-    - left. auto using in_free_subst_lower_eq.
-  Qed.
-
-  Corollary scoped_subst_eq : forall t k (u : T k leaf) x γ1 γ2,
-      scoped S k t γ1 ->
-      scoped (T k) k u γ2 ->
-      scoped S k (t '{k | x ~> u}) (γ1 \\ {{x}} ∪ γ2).
-  Proof.
-    introv St Su. unfold scoped in *.
-    etransitivity. apply freeset_subst_upper_eq. fsetdec.
-  Qed.
-
-  Corollary freeset_subst_lower_neq : forall t k j u x,
-      k <> j ->
-      freeset S j t ⊆
-      freeset S j (t '{k | x ~> u}).
-  Proof.
-    introv neq. intro a.
-    do 2 rewrite <- (free_iff_freeset).
-    now apply in_free_subst_lower_neq.
-  Qed.
-
-  (** ** Substitution of fresh variables *)
-  Theorem subst_fresh : forall t k x u,
-      ~ x ∈ free S k t ->
-      t '{k | x ~> u} = t.
-  Proof.
-    intros. apply (subst_id S). intros.
-    assert (Fr x <> l). admit.
-    now simpl_local.
-  Admitted.
-
-  Corollary subst_fresh_set : forall t k x u,
-      ~ x ∈@ freeset S k t ->
-      t '{k | x ~> u} = t.
-  Proof.
-    setoid_rewrite <- free_iff_freeset. apply subst_fresh.
-  Qed.
-
-  Theorem subst_fresh_t : forall k' (t : T k' leaf) k x u,
-      ~ x ∈ free (T k') k t ->
-      t '{k | x ~> u} = t.
-  Proof.
-    intros. apply (subst_id (T k')). intros.
-    assert (Fr x <> l) by eauto using ninf_in_neq_t.
-    now simpl_local.
-  Qed.
-
-  Corollary subst_fresh_set_t : forall k' (t : T k' leaf) k x u,
-      ~ x ∈@ freeset (T k') k t ->
-      t '{k | x ~> u} = t.
-  Proof.
-    setoid_rewrite <- free_iff_freeset. apply subst_fresh_t.
-  Qed.
-
-  Theorem free_subst_fresh : forall t k j u x,
-      ~ x ∈ free S k t ->
-      free S j (t '{k | x ~> u}) = free S j t.
-  Proof with auto.
-    introv fresh. replace (t '{k | x ~> u}) with t...
-    rewrite subst_fresh...
-  Qed.
-
-  Corollary free_subst_fresh_eq : forall t k u x,
-      ~ x ∈ free S k t ->
-      free S k (t '{k | x ~> u}) = free S k t.
-  Proof.
-    introv fresh. replace (t '{k | x ~> u}) with t; auto.
-    now rewrite subst_fresh.
-  Qed.
-
-  Corollary freeset_subst_fresh : forall t k j u x,
-      ~ x ∈@ freeset S k t ->
-      freeset S j (t '{k | x ~> u}) [=] freeset S j t.
-  Proof.
-    introv fresh. intro y.
-    rewrite <- ?(free_iff_freeset) in *.
-    now rewrite free_subst_fresh.
-  Qed.
-
-  Corollary freeset_subst_fresh_eq : forall t k u x,
-      ~ x ∈@ freeset S k t ->
-      freeset S k (t '{k | x ~> u}) [=] freeset S k t.
-  Proof.
-    intros. apply freeset_subst_fresh; auto.
-  Qed.
-
-  (** ** Composing substitutions *)
-
-
-  Create HintDb tmp.
-  Hint Rewrite @subst_in_mret_neq using auto : tmp.
-       (* using (solve [typeclasses eauto] || auto ] : tea_local. *)
-
-  Lemma subst_subst_neq_loc : forall j k1 k2 (u1 : T k1 leaf) (u2 : T k2 leaf) (x1 x2 : atom),
-      k1 <> k2 ->
-      ~ x1 ∈ free (T k2) k1 u2 ->
-      subst (T j) k2 x2 u2 ∘ btg T k1 (subst_loc k1 x1 u1) j =
-      subst (T j) k1 x1 (subst (T k1) k2 x2 u2 u1) ∘ btg T k2 (subst_loc k2 x2 u2) j.
-  Proof with easy.
-    intros. ext l. unfold compose. compare j to both of { k1 k2 }.
-    - do 2 simpl_tgt_fallback.
-      simpl_local.
-      compare l to atom x1.
-      + rewrite 2(subst_loc_eq)...
-      + rewrite subst_loc_neq; auto. now simpl_local.
-      + rewrite subst_loc_b. now simpl_local.
-    - simpl_tgt. simpl_local. compare l to atom x2.
-      + simpl_local. rewrite subst_fresh_t...
-      + simpl_local...
-      + simpl_local...
-    - simpl_tgt_fallback. now do 2 (rewrite subst_in_mret_neq; auto).
-  Qed.
-
-  Theorem subst_subst_neq : forall k1 k2 u1 u2 t (x1 x2 : atom),
-      k1 <> k2 ->
-      ~ x1 ∈ free (T k2) k1 u2 ->
-      t '{k1 | x1 ~> u1} '{k2 | x2 ~> u2} =
-      t '{k2 | x2 ~> u2} '{k1 | x1 ~> u1 '{k2 | x2 ~> u2} }.
-  Proof.
-    intros. unfold subst.
-    compose near t on left.
-    compose near t on right.
-    unfold kbind. rewrite 2(mbind_mbind S).
-    fequal. ext j. now apply subst_subst_neq_loc.
-  Qed.
-
-  Lemma subst_subst_eq_local : forall k u1 u2 x1 x2,
-      ~ x1 ∈ free (T k) k u2 ->
-      x1 <> x2 ->
-      subst (T k) k x2 u2 ∘ subst_loc k x1 u1 =
-      subst (T k) k x1 (subst (T k) k x2 u2 u1) ∘ subst_loc k x2 u2.
-  Proof with auto.
-    intros. ext l. unfold compose. compare l to atom x1.
-    - rewrite subst_loc_eq, subst_loc_neq,
-      subst_in_mret_eq, subst_loc_eq...
-    - rewrite subst_loc_neq...
-      compare values x2 and a.
-      + rewrite subst_in_mret_eq, subst_loc_eq, subst_fresh_t...
-      + rewrite subst_loc_neq, 2(subst_in_mret_eq), 2(subst_loc_neq)...
-    - rewrite 2(subst_loc_b), 2(subst_in_mret_eq), 2(subst_loc_b)...
-  Qed.
-
-  Theorem subst_subst_eq : forall k u1 u2 t x1 x2,
-      ~ x1 ∈ free (T k) k u2 ->
-      x1 <> x2 ->
-      t '{k | x1 ~> u1} '{k | x2 ~> u2} =
-      t '{k | x2 ~> u2} '{k | x1 ~> u1 '{k | x2 ~> u2} }.
-  Proof with auto.
-    intros. unfold subst.
-    compose near t.
-    rewrite 2(kbind_kbind S).
-    fequal. now apply subst_subst_eq_local.
-  Qed.
-
-  (** ** Commuting two substitutions *)
-  Corollary subst_subst_comm_eq : forall k u1 u2 t x1 x2,
-      x1 <> x2 ->
-      ~ x1 ∈ free (T k) k u2 ->
-      ~ x2 ∈ free (T k) k u1 ->
-      t '{k | x1 ~> u1} '{k | x2 ~> u2} =
-      t '{k | x2 ~> u2} '{k | x1 ~> u1}.
-  Proof.
-    intros. rewrite subst_subst_eq; auto.
-    rewrite subst_fresh_t; auto.
-  Qed.
-
-  Corollary subst_subst_comm_neq : forall k1 k2 u1 u2 t x1 x2,
-      k1 <> k2 ->
-      ~ x1 ∈ free (T k2) k1 u2 ->
-      ~ x2 ∈ free (T k1) k2 u1 ->
-      t '{k1 | x1 ~> u1} '{k2 | x2 ~> u2} =
-      t '{k2 | x2 ~> u2} '{k1 | x1 ~> u1}.
-  Proof.
-    intros. rewrite subst_subst_neq; auto.
-    rewrite subst_fresh_t; auto.
-  Qed.
-
-  (** ** Local closure is preserved by substitution *)
-  Theorem subst_lc_eq : forall k u t x,
-      locally_closed S k t ->
-      locally_closed (T k) k u ->
-      locally_closed S k (subst S k x u t).
-  Proof.
-    unfold locally_closed. introv lct lcu hin.
-    rewrite ind_subst_iff_eq in hin.
-    destruct hin as [[? ?] | [n1 [n2 [h1 [h2 h3]]]]].
-    - auto.
-    - subst. specialize (lcu n2 l h2).
-      unfold is_bound_or_free in *.
-      destruct l; auto. unfold_monoid.
-      rewrite countk_app. lia.
-  Qed.
-
-  Theorem subst_lc_neq : forall k j u t x,
-      k <> j ->
-      locally_closed S j t ->
-      locally_closed (T k) j u ->
-      locally_closed S j (subst S k x u t).
-  Proof.
-    unfold locally_closed. introv neq lct lcu hin.
-    rewrite ind_subst_iff_neq in hin; auto.
-    destruct hin as [? | [n1 [n2 [h1 [h2 h3]]]]].
-    - auto.
-    - subst. specialize (lcu n2 l h2).
-      unfold is_bound_or_free in *.
-      destruct l; auto. unfold_monoid.
-      rewrite countk_app. lia.
-  Qed.
-
-  (** ** Decompose substitution into closing/opening *)
-  Lemma subst_spec_local : forall k u w l x,
-      subst_loc k x u l =
-      open_loc k u (w, (close_loc k x) (w, l)).
-  Proof.
-  Admitted.
-  (*
-    introv. compare l to atom x; autorewrite* with tea_local.
-    - cbn. compare values x and x. unfold id.
-      compare naturals (w k) and (w k).
-    - cbn. compare values x and a. (* todo fix fragile names *)
-    - cbn. unfold id. compare naturals n and (w k).
-      now compare naturals (S (w k)) and (w k).
-      now compare naturals (S n) and (w k).
-  Qed.
-*)
-
-  Theorem subst_spec : forall k x u t,
-      t '{k | x ~> u} = ('[k | x] t) '(k | u).
-  Proof.
-  Admitted.
-  (*
-    intros. compose near t on right.
-    unfold open, close, subst.
-    rewrite (kbindd_kfmapd F).
-    symmetry. apply (kbindr_proper_kbind S k t).
-    symmetry. apply subst_spec_local.
-  Qed.
-*)
-
-  (** ** Substitution when <<u>> is a leaf **)
-  Definition subst_loc_leaf k x (u : leaf) : leaf -> leaf :=
-    fun l => match l with
-          | Fr y => if x == y then u else Fr y
-          | Bd n => Bd n
-          end.
-
-  Theorem subst_by_leaf_spec : forall k x l,
-      subst S k x (mret T k l) = kfmap S k (subst_loc_leaf k x l).
-  Proof.
-    intros. unfold subst. ext t.
-    apply kbind_respectful_kfmap.
-    intros l' Hin. destruct l'.
-    - cbn. compare values x and a.
-    - reflexivity.
-  Qed.
-
-  (** ** Substitution by the same variable is the identity *)
-  (** TODO : Intuitively this theorem should be stronger, but
-      this is because we don't have strong properness for [bind] in general. *)
-  Theorem subst_same : forall t k x,
-      t '{k | x ~> mret T k (Fr x)} = t.
-  Proof.
-    intros. apply (subst_id S).
-    intros. compare l to atom x; now simpl_local.
-  Qed.
-
   (** ** Free variables after variable closing *)
+  (******************************************************************************)
   Lemma in_free_close_iff_loc_1 : forall k w l t x  y,
       (w, k, l) ∈md t ->
       Fr y = close_loc k x (w, l) ->
@@ -875,25 +1181,22 @@ Section locally_nameless_metatheory.
   Qed.
 
   (** ** Variable closing and local closure *)
+  (******************************************************************************)
   Theorem close_lc_eq : forall k t x,
       locally_closed S k t ->
       locally_closed_gap S k 1 (close S k x t).
   Proof.
     unfold locally_closed. introv lct hin.
-    rewrite ind_close_iff_eq in hin.
+    rewrite (ind_close_iff_eq S) in hin.
     destruct hin as [l1 [? ?]]. compare l1 to atom x; subst.
-    - cbn. compare values x and x. unfold_lia.
+    - cbn. compare values x and x. unfold_monoid; lia.
     - cbn. compare values x and a.
     - cbn. compare naturals n and (countk k w).
-      (*
-      + admit.
-      + (* contradiction *)
-        specialize (lct w (Bd (w k)) ltac:(assumption)).
-        cbn in lct. now unfold_lia.
+      + specialize (lct w (Bd (countk k w)) ltac:(assumption)).
+        cbn in lct. now unfold_monoid; lia.
       + specialize (lct w (Bd n) ltac:(assumption)).
-        cbn in lct. now unfold_lia.
-*)
-  Admitted.
+        cbn in lct. now unfold_monoid; lia.
+  Qed.
 
   Theorem close_lc_neq : forall k j t x,
       k <> j ->
@@ -904,17 +1207,35 @@ Section locally_nameless_metatheory.
     rewrite (ind_close_neq_iff S) in hin; auto.
   Qed.
 
+End close_metatheory.
+
+(** ** Metatheory for <<open>> *)
+(******************************************************************************)
+Section open_metatheory.
+
+  Context
+    (S : Type -> Type)
+    `{DTPreModule (list K) S T (mn_op := Monoid_op_list) (mn_unit := Monoid_unit_list)}
+    `{! DTM (list K) T}.
+
+  Implicit Types
+           (k : K) (j : K)
+           (l : leaf) (p : leaf)
+           (x : atom) (t : S leaf)
+           (w : list K) (n : nat).
+
   (** ** Upper and lower bounds on free variables after opening *)
+  (******************************************************************************)
   Lemma free_open_upper_local : forall t k j (u : T k leaf) w l x,
       (k, l) ∈m t ->
       x ∈ free (T k) j (open_loc k u (w, l)) ->
-        k = j /\ l = Fr x /\ x ∈ free S j t \/
-        x ∈ free (T k) j u.
-    Proof with auto.
-      introv lin xin. rewrite in_free_iff_T in xin.
-      rewrite 2(in_free_iff). destruct l as [y | n].
-      - left. autorewrite with tea_local in xin. inverts xin...
-      - right. cbn in xin. compare naturals n and (countk k w).
+      k = j /\ l = Fr x /\ x ∈ free S j t \/
+      x ∈ free (T k) j u.
+  Proof with auto.
+    introv lin xin. rewrite in_free_iff in xin.
+    rewrite 2(in_free_iff). destruct l as [y | n].
+    - left. autorewrite with tea_local in xin. inverts xin...
+    - right. cbn in xin. compare naturals n and (countk k w).
       { contradict xin. simpl_local. intuition. }
       { assumption. }
       { contradict xin. simpl_local. intuition. }
@@ -922,7 +1243,7 @@ Section locally_nameless_metatheory.
 
   Corollary free_open_upper_local_eq : forall t k (u : T k leaf) w l x,
       (k, l) ∈m t ->
-      x ∈ free (T k) k (open_loc u (w, l)) ->
+      x ∈ free (T k) k (open_loc k u (w, l)) ->
       x ∈ free S k t \/ x ∈ free (T k) k u.
   Proof.
     introv lin xin.
@@ -934,7 +1255,7 @@ Section locally_nameless_metatheory.
   Corollary free_open_upper_local_neq : forall t k j (u : T k leaf) w l x,
       k <> j ->
       (k, l) ∈m t ->
-      x ∈ free (T k) j (open_loc u (w, l)) ->
+      x ∈ free (T k) j (open_loc k u (w, l)) ->
       x ∈ free (T k) j u.
   Proof.
     introv neq lin xin.
@@ -948,13 +1269,13 @@ Section locally_nameless_metatheory.
       x ∈ free S j t \/ x ∈ free (T k) j u.
   Proof.
     introv xin. compare values j and k.
-    - rewrite free_open_iff_eq in xin.
-      destruct xin as [l [w [hin ?]]].
-      apply (in_of_ind F) in hin.
+    - rewrite (free_open_eq_iff S) in xin.
+      destruct xin as [w [l [hin ?]]].
+      eapply (ind_implies_in S) in hin.
       eauto using free_open_upper_local_eq.
-    - rewrite free_open_iff_neq in xin; auto.
-      destruct xin as  [? |  [l [w [hin ?]]]].
-      auto. apply (in_of_ind F) in hin.
+    - rewrite (free_open_neq_iff S) in xin; auto.
+      destruct xin as  [? |  [w [l [hin ?]]]].
+      auto. apply (ind_implies_in S) in hin.
       right. eauto using free_open_upper_local_neq.
   Qed.
 
@@ -985,12 +1306,12 @@ Section locally_nameless_metatheory.
   Proof.
     introv xin. compare values j and k.
     - rewrite (in_free_iff) in xin.
-      rewrite (ind_of_in F) in xin.
+      rewrite (ind_iff_in S) in xin.
       destruct xin as [w xin].
-      rewrite (free_open_iff_eq k).
+      rewrite (free_open_eq_iff S).
       setoid_rewrite (in_free_iff).
-      exists (Fr x) w. now autorewrite with tea_local.
-    - rewrite (free_open_iff_neq k); auto.
+      exists w (Fr x). now autorewrite with tea_local.
+    - rewrite (free_open_neq_iff S); auto.
   Qed.
 
   Theorem free_open_lower_eq : forall t k u x,
@@ -1017,46 +1338,45 @@ Section locally_nameless_metatheory.
   (**************************************************************************)
   Lemma open_lc_local : forall k (u : T k leaf) w l,
       is_bound_or_free k 0 (w, l) ->
-      open_loc u (w, l) = mret T k l.
+      open_loc k u (w, l) = mret T k l.
   Proof.
     introv hyp. destruct l as [a | n].
     - reflexivity.
-    - cbn in *. compare naturals n and (w k); unfold_lia.
+    - cbn in *. compare naturals n and (countk k w); unfold_monoid; lia.
   Qed.
 
   Lemma open_lc : forall k t u,
       locally_closed S k t ->
       t '(k | u) = t.
   Proof.
-    introv lc. apply open_id. introv lin.
+    introv lc. apply (open_id S). introv lin.
     specialize (lc _ _ lin).
     destruct l; auto using open_lc_local.
   Qed.
 
   (** ** Opening followed by substitution *)
   (**************************************************************************)
-  Open Scope nat_scope.
-
   Lemma subst_open_eq_loc : forall k u1 u2 x,
       locally_closed (T k) k u2 ->
-      subst (T k) k x u2 ∘ open_loc u1 =
-      open_loc (u1 '{k | x ~> u2}) ∗kr (subst_loc x u2 ∘ snd).
+      subst (T k) k x u2 ∘ open_loc k u1 =
+      open_loc k (u1 '{k | x ~> u2}) ⋆kdm (subst_loc k x u2 ∘ snd).
   Proof.
-    introv lcu2. ext [w l]. rewrite kcompkr_spec.
+    introv lcu2. ext [w l]. unfold compose_kdm.
     unfold compose. compare l to atom x.
     - cbn. simpl_local. compare values x and x.
-      symmetry. apply (kbindr_proper_id (T k)). intros ? [?|?] hin.
+      symmetry. apply kbindd_respectful_id. intros ? [?|?] hin.
       + trivial.
       + specialize (lcu2 _ _ hin). cbn in lcu2. cbn. unfold_monoid.
-        compare naturals n and (w k + w0 k).
+        rewrite countk_app.
+        compare naturals n and (countk k w + countk k w0).
     - cbn. simpl_local. compare values x and a.
-      now rewrite (kbindr_comp_mret_eq (T k) k).
-      (* <<< TODO standardize this lemma *)
-    - cbn. rewrite (kbindr_comp_mret_eq (T k) k).
-      compare naturals n and (w k); simpl_local.
-      + rewrite monoid_id_l. cbn. compare naturals n and (w k).
-      + rewrite monoid_id_l. cbn. compare naturals (w k) and (w k).
-      + rewrite monoid_id_l. cbn. compare naturals n and (w k).
+      now rewrite (kbindd_comp_mret_eq).
+    (* <<< TODO standardize this lemma *)
+    - cbn. rewrite (kbindd_comp_mret_eq).
+      compare naturals n and (countk k w); cbn; simpl_local.
+      + rewrite monoid_id_l. compare naturals n and (countk k w).
+      + rewrite monoid_id_l. cbn. compare naturals (countk k w) and (countk k w).
+      + rewrite monoid_id_l. cbn. compare naturals n and (countk k w).
   Qed.
 
   Theorem subst_open_eq :  forall k u1 u2 t x,
@@ -1066,24 +1386,11 @@ Section locally_nameless_metatheory.
   Proof.
     introv lc. compose near t.
     unfold open, subst at 1 3.
-    rewrite (kbind_kbindr F), (kbindr_kbind F).
+    rewrite (kbind_kbindd S), (kbindd_kbind S).
     fequal. apply subst_open_eq_loc; auto.
   Qed.
 
   (*
-  Theorem subst_open_neq :  forall j k u1 u2 t x,
-      k <> j ->
-      locally_closed k u2 ->
-      t '(k | u1) '{j | x ~> u2} =
-      t '{j | x ~> u2} '(k | u1 '{j | x ~> u2}).
-  Proof.
-    introv neq lc. compose near t.
-    unfold open, subst at 1 3.
-    rewrite (kbind_kbindr F). (kbindr_kbind F).
-    fequal. apply subst_open_loc; auto.
-  Qed.
-   *)
-
   Lemma subst_open_neq_loc k1 k2 (u1 : T k1 leaf) (u2 : T k2 leaf) (x : atom) :
     k1 <> k2 ->
     locally_closed (T k2) k1 u2 ->
@@ -1136,19 +1443,20 @@ Section locally_nameless_metatheory.
     rewrite (mbind_mbindr F), (mbindr_mbind F).
     fequal. now rewrite subst_open_neq_loc.
   Qed.
+   *)
 
   (** ** Decompose opening into variable opening followed by substitution *)
   (**************************************************************************)
   Lemma open_spec_eq_loc : forall k u x w l,
       l <> Fr x ->
-      (subst (T k) k x u ∘ open_loc (mret T k (Fr x))) (w, l) =
-      open_loc u (w, l).
+      (subst (T k) k x u ∘ open_loc k (mret T k (Fr x))) (w, l) =
+      open_loc k u (w, l).
   Proof.
     introv neq. unfold compose. compare l to atom x.
     - contradiction.
     - cbn. rewrite subst_in_mret_eq, subst_loc_fr_neq.
       trivial. intuition.
-    - cbn. compare naturals n and (w k).
+    - cbn. compare naturals n and (countk k w).
       now rewrite subst_in_mret_eq.
       now rewrite subst_in_mret_eq, subst_loc_eq.
       now rewrite subst_in_mret_eq, subst_loc_b.
@@ -1162,10 +1470,10 @@ Section locally_nameless_metatheory.
       t '(k | u) = t '(k | mret T k (Fr x)) '{k | x ~> u}.
   Proof.
     introv fresh. compose near t on right.
-    unfold subst, open. rewrite (kbind_kbindr F).
-    apply (kbindr_proper F). intros.
+    unfold subst, open. rewrite (kbind_kbindd S).
+    apply (kbindd_respectful). introv Hin.
     assert (a <> Fr x).
-    { apply (in_of_ind F) in H5.
+    { apply (ind_implies_in S) in Hin.
       rewrite <- free_iff_freeset in fresh.
       eapply ninf_in_neq in fresh; eauto. }
     now rewrite <- (open_spec_eq_loc k u x).
@@ -1176,8 +1484,8 @@ Section locally_nameless_metatheory.
   Lemma subst_open_var_loc : forall k u x y,
       x <> y ->
       locally_closed (T k) k u ->
-      subst (T k) k x u ∘ open_loc (mret T k (Fr y)) =
-      open_loc (mret T k (Fr y)) ∗kr (subst_loc x u ∘ snd).
+      subst (T k) k x u ∘ open_loc k (mret T k (Fr y)) =
+      open_loc k (mret T k (Fr y)) ⋆kdm (subst_loc k x u ∘ extract (prod (list K))).
   Proof with auto.
     introv neq lc. rewrite subst_open_eq_loc...
     simpl_local. reflexivity.
@@ -1191,22 +1499,22 @@ Section locally_nameless_metatheory.
   Proof.
     introv neq lc. compose near t.
     unfold open, subst.
-    rewrite (kbind_kbindr F), (kbindr_kbind F).
+    rewrite (kbind_kbindd S), (kbindd_kbind S).
     fequal. apply subst_open_var_loc; auto.
   Qed.
 
   (** ** Closing, followed by opening *)
   (**************************************************************************)
   Lemma open_close_loc : forall k x w l,
-      (open_loc (mret T k (Fr x)) ∘ cobind (prod (Row nat))
+      (open_loc k (mret T k (Fr x)) ∘ cobind (prod (list K))
                 (close_loc k x)) (w, l) = mret T k l.
   Proof.
     intros. cbn. unfold id. compare l to atom x.
-    - compare values x and x. compare naturals (w k) and (w k).
+    - compare values x and x. compare naturals (countk k w) and (countk k w).
     - compare values x and a.
-    - compare naturals n and (w k).
-      compare naturals (S (w k)) and (w k).
-      compare naturals (S n) and (w k).
+    - compare naturals n and (countk k w).
+      compare naturals (Datatypes.S (countk k w)) and (countk k w).
+      compare naturals (Datatypes.S n) and (countk k w).
   Qed.
 
   Theorem open_close : forall k x t,
@@ -1214,49 +1522,51 @@ Section locally_nameless_metatheory.
   Proof.
     intros. compose near t on left.
     unfold open, close.
-    rewrite (kbindr_kfmapr F).
-    apply (kbindr_proper_id F); intros.
-    auto using open_close_loc.
+    rewrite (kbindd_kfmapd S).
+    apply (kbindd_respectful_id); intros.
+    apply open_close_loc.
   Qed.
 
-  (** ** Opening by a leaf reduces to an [kfmapr] *)
-  Definition open_leaf_loc k (u : leaf) : Row nat * leaf -> leaf :=
-    fun wl => match wl with
-           | (w, l) =>
-             match l with
-             | Fr x => Fr x
-             | Bd n =>
-               match Nat.compare n (w k) with
-               | Gt => Bd (n - 1)
-               | Eq => u
-               | Lt => Bd n
-               end
-             end
-           end.
+  (** ** Opening by a leaf reduces to an [kfmapd] *)
+  (**************************************************************************)
+  Definition open_leaf_loc k (u : leaf) : list K * leaf -> leaf :=
+    fun wl =>
+      match wl with
+      | (w, l) =>
+        match l with
+        | Fr x => Fr x
+        | Bd n =>
+          match Nat.compare n (countk k w) with
+          | Gt => Bd (n - 1)
+          | Eq => u
+          | Lt => Bd n
+          end
+        end
+      end.
 
   Lemma open_by_leaf_spec : forall k l,
-      open S k (mret T k l) = kfmapr S k (open_leaf_loc k l).
+      open S k (mret T k l) = kfmapd S k (open_leaf_loc k l).
   Proof.
     intros. unfold open. ext t.
-    apply (kbindr_proper_kfmapr F).
+    apply (kbindd_respectful_kfmapd).
     intros w l' l'in. destruct l'.
     - reflexivity.
-    - cbn. compare naturals n and (w k).
+    - cbn. compare naturals n and (countk k w).
   Qed.
 
   (** ** Opening, followed by closing *)
   (**************************************************************************)
   Lemma close_open_local : forall k x w l,
       l <> Fr x ->
-      (close_loc k x ∘ cobind (prod (Row nat))
+      (close_loc k x ∘ cobind (prod (list K))
                  (open_leaf_loc k (Fr x))) (w, l) = l.
   Proof.
     introv neq. cbn. unfold id. compare l to atom x.
     - contradiction.
     - unfold compose; cbn. now compare values x and a.
     - unfold compose; cbn.
-      compare naturals n and (w k). compare values x and x.
-      compare naturals (n - 1) and (w k).
+      compare naturals n and (countk k w). compare values x and x.
+      compare naturals (n - 1) and (countk k w).
   Qed.
 
   Theorem close_open : forall k x t,
@@ -1265,13 +1575,13 @@ Section locally_nameless_metatheory.
   Proof.
     introv fresh. compose near t on left.
     rewrite open_by_leaf_spec. unfold close.
-    rewrite (kfmapr_kfmapr_eq S k).
-    apply (kfmapr_proper_id F).
+    rewrite (kfmapd_kfmapd S).
+    apply (kfmapd_respectful_id).
     intros w l lin.
     assert (l <> Fr x).
-    { rewrite neq_symmetry. apply (in_of_ind F) in lin.
-      eauto using ninf_in_neq. }
-    auto using close_open_local.
+    { rewrite neq_symmetry. apply (ind_implies_in) in lin.
+      eapply (ninf_in_neq S). eassumption. auto. }
+    now apply close_open_local.
   Qed.
 
   (** ** Opening and local closure *)
@@ -1282,18 +1592,18 @@ Section locally_nameless_metatheory.
       locally_closed_gap S k (n - 1) (t '(k | u)).
   Proof.
     unfold locally_closed_gap.
-    introv lcu lct Hin. rewrite ind_open_iff_eq in Hin.
-    destruct Hin as [l1 [n1 [n2 [h1 [h2 h3]]]]].
+    introv lcu lct Hin. rewrite (ind_open_iff_eq S) in Hin.
+    destruct Hin as [w1 [w2 [l1 [h1 [h2 h3]]]]].
     destruct l1.
-    - cbn in h2. rewrite ind_mret_iff_eq in h2.
+    - cbn in h2. rewrite ind_mret_eq_iff in h2.
       destruct h2; subst. cbn. trivial.
-    - specialize (lct _ _ h1). cbn in h2. compare naturals n0 and (n1 k).
-      + rewrite ind_mret_iff_eq in h2; destruct h2; subst.
-        cbn. unfold_monoid. lia.
-      + specialize (lcu n2 l h2). unfold is_bound_or_free in *.
-        destruct l; [trivial|]. unfold_monoid. lia.
-      + rewrite ind_mret_iff_eq in h2. destruct h2; subst.
-        unfold is_bound_or_free in *. unfold_lia.
+    - specialize (lct _ _ h1). cbn in h2. compare naturals n0 and (countk k w1).
+      + rewrite ind_mret_eq_iff in h2; destruct h2; subst.
+        cbn. unfold_monoid. List.simpl_list. lia.
+      + specialize (lcu w2 l h2). unfold is_bound_or_free in *.
+        destruct l; [trivial|]. unfold_monoid. rewrite countk_app. lia.
+      + rewrite ind_mret_eq_iff in h2. destruct h2; subst.
+        unfold is_bound_or_free in *. unfold_monoid. List.simpl_list. lia.
   Qed.
 
   Lemma open_lc_gap_eq_2 : forall k n t u,
@@ -1303,23 +1613,23 @@ Section locally_nameless_metatheory.
       locally_closed_gap S k n t.
   Proof.
     unfold locally_closed_gap.
-    introv ngt lcu lct Hin. setoid_rewrite ind_open_iff_eq in lct.
+    introv ngt lcu lct Hin. setoid_rewrite (ind_open_iff_eq S) in lct.
     destruct l.
     - cbv. trivial.
-    - compare naturals n0 and (w k).
+    - compare naturals n0 and (countk k w).
       + specialize (lct w (Bd n0)).
         lapply lct.
-        { cbn; unfold_lia. }
-        { exists (Bd n0) w (Ƶ : Row nat).
-          split; auto. cbn. compare naturals n0 and (w k).
-          rewrite ind_mret_iff_eq. now simpl_monoid. }
-      + cbn. unfold_lia.
+        { cbn; unfold_monoid; lia. }
+        { exists w (Ƶ : list K) (Bd n0).
+          split; auto. cbn. compare naturals n0 and (countk k w).
+          rewrite ind_mret_eq_iff. now simpl_monoid. }
+      + cbn. unfold_monoid; lia.
       + cbn. specialize (lct w (Bd (n0 - 1))).
         lapply lct.
-        { cbn; unfold_lia. }
-        { exists (Bd n0) w (Ƶ : Row nat).
-          split; auto. cbn. compare naturals n0 and (w k).
-          rewrite ind_mret_iff_eq. now simpl_monoid. }
+        { cbn; unfold_monoid; lia. }
+        { exists w (Ƶ : list K) (Bd n0).
+          split; auto. cbn. compare naturals n0 and (countk k w).
+          rewrite ind_mret_eq_iff. now simpl_monoid. }
   Qed.
 
   Theorem open_lc_gap_eq_iff : forall k n t u,
@@ -1337,7 +1647,7 @@ Section locally_nameless_metatheory.
       locally_closed_gap S k (n - 1) (t '(k | mret T k (Fr x))).
   Proof.
     intros. apply open_lc_gap_eq_iff. auto.
-    intros w l hin. rewrite ind_mret_iff_eq in hin.
+    intros w l hin. rewrite ind_mret_eq_iff in hin.
     destruct hin; subst. cbv. trivial.
   Qed.
 
@@ -1370,20 +1680,21 @@ Section locally_nameless_metatheory.
   Proof.
     unfold locally_closed_gap.
     introv neq lcu lct Hin.
-    rewrite ind_open_iff_neq in Hin; auto.
-    destruct Hin.
+    rewrite (ind_open_neq_iff S) in Hin; auto.
+    destruct Hin as [Hin | Hin].
     - auto.
-    - destruct H5 as [l' [n1 [n2 [in_t [in_open ?]]]]].
-      subst. destruct l'.
+    - destruct Hin as [w1 [w2 [l1 [in_t [in_open ?]]]]].
+      subst. destruct l1.
       + cbn in in_open. rewrite ind_mret_iff in in_open.
         false. intuition.
       + destruct l.
         { cbn. trivial. }
         { cbn. cbn in in_open.
-          compare naturals n0 and (n1 j).
+          compare naturals n0 and (countk j w1).
           - rewrite ind_mret_iff in in_open. false; intuition.
           - specialize (lcu _ _ in_open).
-            unfold is_bound_or_free in lcu. unfold_lia.
+            unfold is_bound_or_free in lcu. unfold_monoid.
+            rewrite countk_app. lia.
           - rewrite ind_mret_iff in in_open. false; intuition.
         }
   Qed.
@@ -1399,7 +1710,7 @@ Section locally_nameless_metatheory.
     destruct l.
     + cbn. auto.
     + specialize (lct w (Bd n0)).
-      apply lct. rewrite ind_open_iff_neq; auto.
+      apply lct. rewrite (ind_open_neq_iff S); auto.
   Qed.
 
   Theorem open_lc_gap_neq_iff : forall k j n t u,
@@ -1422,4 +1733,17 @@ Section locally_nameless_metatheory.
     setoid_rewrite ind_mret_iff. intuition.
   Qed.
 
-End locally_nameless_metatheory.
+End open_metatheory.
+
+(*
+
+  Corollary scoped_subst_eq : forall t k (u : T k leaf) x γ1 γ2,
+      scoped S k t γ1 ->
+      scoped (T k) k u γ2 ->
+      scoped S k (t '{k | x ~> u}) (γ1 \\ {{x}} ∪ γ2).
+  Proof.
+    introv St Su. unfold scoped in *.
+    etransitivity. apply freeset_subst_upper_eq. fsetdec.
+  Qed.
+
+*)
