SystemF/Contexts.v
@@ -1,0 +1,615 @@
+From Tealeaves Require Import
+     Functors.List
+     LN.Leaf LN.Atom LN.AtomSet LN.AssocList
+     LN.Multisorted.Operations.
+
+From Multisorted Require Import
+     Classes.DTM.
+
+From Coq Require Import
+     Sorting.Permutation.
+
+From Tealeaves.Examples Require Import
+     SystemF.Language.
+
+Implicit Types (x : atom).
+
+Import List.ListNotations.
+Import LN.AssocList.Notations.
+
+Create HintDb sysf_ctx.
+
+(** * Tactical support *)
+(******************************************************************************)
+Ltac burst :=
+  rewrite_strat
+    outermost
+    (choice (hints tea_rw_dom)
+            (choice (hints tea_rw_range)
+                    (choice (hints tea_rw_disj)
+                            (choice (hints tea_rw_uniq)
+                                    (hints tea_list))))).
+
+Tactic Notation "burst" "in" hyp(H) :=
+  rewrite_strat
+    outermost
+    (choice (hints tea_rw_dom)
+            (choice (hints tea_rw_range)
+                    (choice (hints tea_rw_disj)
+                            (choice (hints tea_rw_uniq)
+                                    (hints tea_list))))) in H.
+
+Tactic Notation "bursts" :=
+  repeat match goal with
+         | H : _ |- _ => burst in H
+         end; repeat burst.
+
+(** * Infrastructural lemmas for contexts and well-formedness predicates *)
+(******************************************************************************)
+
+(** ** Reasoning principle for scope (<<scoped>>) *)
+(******************************************************************************)
+Section scope_lemmas.
+
+  Context
+    (S : Type -> Type)
+    `{DTPreModule (list K) S T (mn_op := Monoid_op_list) (mn_unit := Monoid_unit_list)}
+    `{! DTM (list K) T}.
+
+  Theorem perm_scoped : forall (t : S leaf) (X : Type) (γ1 γ2 : alist X) (k : K),
+      Permutation γ1 γ2 ->
+      scoped S k t (domset γ1) ->
+      scoped S k t (domset γ2).
+  Proof.
+    introv Hperm. unfold scoped. rewrite (perm_domset); eauto.
+  Qed.
+
+  Theorem perm_scoped_iff : forall (t : S leaf) (X : Type) (γ1 γ2 : alist X) (k : K),
+      Permutation γ1 γ2 ->
+      scoped S k t (domset γ1) <->
+      scoped S k t (domset γ2).
+  Proof.
+    intros. assert (Permutation γ2 γ1) by now symmetry.
+    split; eauto using perm_scoped.
+  Qed.
+
+  Lemma weak_scoped_app_l : forall (t : S leaf) (X : Type) (γ1 γ2 : alist X) (k : K),
+      scoped S k t (domset γ1) ->
+      scoped S k t (domset (γ1 ++ γ2)).
+  Proof.
+    intros. unfold scoped in *.
+    autorewrite with tea_rw_dom. fsetdec.
+  Qed.
+
+  Lemma weak_scoped_app_r : forall (t : S leaf) (X : Type) (γ1 γ2 : alist X) (k : K),
+      scoped S k t (domset γ2) ->
+      scoped S k t (domset (γ1 ++ γ2)).
+  Proof.
+    intros. unfold scoped in *.
+    autorewrite with tea_rw_dom. fsetdec.
+  Qed.
+
+  Lemma strengthen_scoped : forall (t : S leaf) (X : Type) (γ1 γ2 : alist X) (k : K) (x : atom) (x' : X),
+      scoped S k t (domset (γ1 ++ x ~ x' ++ γ2)) ->
+      ~ x ∈@ (freeset S k t) ->
+      scoped S k t (domset (γ1 ++ γ2)).
+  Proof.
+    introv hyp hnotin. unfold scoped in *.
+    autorewrite with tea_rw_dom in *. fsetdec.
+  Qed.
+
+  Lemma sub_scoped :
+    forall (t1 : S leaf) (k : K) (t2 : T k leaf)
+      (X : Type) (γ1 γ2 : alist X) (x : atom) (x' : X),
+      scoped S k t1 (domset (γ1 ++ x ~ x' ++ γ2)) ->
+      scoped (T k) k t2 (domset (γ1 ++ γ2)) ->
+      scoped S k (subst S k x t2 t1) (domset (γ1 ++ γ2)).
+  Proof.
+    introv hyp1 hyp2. unfold scoped in *. autorewrite with tea_rw_dom in *.
+    etransitivity.
+    (*
+      apply freeset_subst_upper_eq. fsetdec.
+     *)
+  Abort.
+
+  Lemma sub_scoped_1 :
+    forall (t1 : S leaf) (k : K) (t2 : T k leaf)
+      (X : Type) (γ1 γ2 : alist X) (x : atom) (x' : X),
+      scoped S k t1 (domset (γ1 ++ x ~ x')) ->
+      scoped (T k) k t2 (domset γ1) ->
+      scoped S k (subst S k x t2 t1) (domset γ1).
+  Proof.
+    (*
+    introv hyp1 hyp2. change_alist (γ ++ x ~ tt ++ []) in hyp1.
+    change_alist (γ ++ []) in hyp2.
+    change_alist (γ ++ []).
+    eauto using sub_scoped.
+     *)
+  Abort.
+
+End scope_lemmas.
+
+(** ** Contexts of type variables (<<ok_tyv>>) *)
+(******************************************************************************)
+Lemma perm_ok_tyv : forall Δ1 Δ2,
+    ok_tyv Δ1 ->
+    Permutation Δ1 Δ2 ->
+    ok_tyv Δ2.
+Proof.
+  unfold ok_tyv. intros. rewrite <- uniq_perm; eauto.
+Qed.
+
+#[export] Hint Immediate perm_ok_tyv : sysf_ctx.
+
+Corollary perm_ok_tyv_iff : forall Δ1 Δ2,
+    Permutation Δ1 Δ2 ->
+    ok_tyv Δ1 <-> ok_tyv Δ2.
+Proof.
+  unfold ok_tyv. intros. now rewrite uniq_perm.
+Qed.
+
+Lemma ok_tyv_nil : forall x,
+    ok_tyv [].
+Proof.
+  intros. unfold ok_tyv in *.
+  now bursts.
+Qed.
+
+#[export] Hint Resolve ok_tyv_nil : sysf_ctx.
+
+Lemma ok_tyv_one : forall x,
+    ok_tyv (x ~ tt).
+Proof.
+  intros. unfold ok_tyv in *.
+  now bursts.
+Qed.
+
+#[export] Hint Resolve ok_tyv_one : sysf_ctx.
+
+Lemma ok_tyv_app_iff : forall Δ1 Δ2,
+    ok_tyv (Δ1 ++ Δ2) <->
+    ok_tyv Δ1 /\ ok_tyv Δ2 /\ disjoint Δ1 Δ2.
+Proof.
+  intros. unfold ok_tyv in *.
+  now bursts.
+Qed.
+
+Lemma ok_tyv_app_1 : forall Δ1 Δ2,
+    ok_tyv Δ1 /\ ok_tyv Δ2 /\ disjoint Δ1 Δ2 ->
+    ok_tyv (Δ1 ++ Δ2).
+Proof.
+  intros. unfold ok_tyv in *.
+  now bursts.
+Qed.
+
+#[export] Hint Resolve ok_tyv_app_1 : sysf_ctx.
+
+Lemma ok_tyv_mid_1: forall Δ1 Δ2 Δ3,
+    ok_tyv (Δ1 ++ Δ2 ++ Δ3) ->
+    ok_tyv Δ2.
+Proof.
+  intros. unfold ok_tyv in *.
+  now bursts.
+Qed.
+
+Lemma ok_tyv_mid_2 : forall Δ1 Δ2 Δ3,
+    ok_tyv (Δ1 ++ Δ2 ++ Δ3) ->
+    ok_tyv (Δ1 ++ Δ3).
+Proof.
+  intros. unfold ok_tyv in *.
+  bursts. now rewrite disjoint_sym.
+Qed.
+
+Lemma ok_tyv_app_l : forall Δ1 Δ2,
+    ok_tyv (Δ1 ++ Δ2) ->
+    ok_tyv Δ1.
+Proof.
+  intros. unfold ok_tyv in *.
+  now bursts.
+Qed.
+
+Lemma ok_tyv_app_r : forall Δ1 Δ2,
+    ok_tyv (Δ1 ++ Δ2) ->
+    ok_tyv Δ2.
+Proof.
+  intros. unfold ok_tyv in *.
+  now bursts.
+Qed.
+
+#[export] Hint Immediate ok_tyv_mid_1 ok_tyv_mid_2 : sysf_ctx.
+#[export] Hint Immediate ok_tyv_app_l ok_tyv_app_r : sysf_ctx.
+
+(** ** Well-scoped types in context Δ *)
+(** A type is well-scoped in a type-variable environment when all of
+    its free variables (which are always type variables) are declared
+    in the context. Such a type may or may not be locally
+    closed. Well-scopedness is preserved under permutation, weakening,
+    and strengthening. It also satisfies a substitution lemma. *)
+(******************************************************************************)
+(*
+(** The <<scoped_type>> predicate supports permutation in Δ. *)
+Lemma perm_scoped_type : forall Δ1 Δ2 τ,
+    Permutation Δ1 Δ2 ->
+    scoped_type Δ1 τ <->
+    scoped_type Δ2 τ.
+Proof.
+  intros. unfold scoped_type. apply perm_scoped_iff; auto.
+Qed.
+
+(** The <<scoped_type>> predicate supports weakening in Δ. *)
+Lemma weak_scoped_type_r : forall Δ1 Δ2 τ,
+    scoped_type Δ1 τ ->
+    scoped_type (Δ1 ++ Δ2) τ.
+Proof.
+  intros. unfold scoped_type in *.
+  now apply weak_scoped_app_l.
+Qed.
+
+Lemma weak_scoped_type_l : forall Δ1 Δ2 τ,
+    scoped_type Δ2 τ ->
+    scoped_type (Δ1 ++ Δ2) τ.
+Proof.
+  intros. unfold scoped_type in *.
+  now apply weak_scoped_app_r.
+Qed.
+
+(** The <<scoped_type>> predicate supports strengthening in Δ for fresh variables. *)
+Lemma stren_scoped_type : forall Δ1 Δ2 x τ,
+    scoped_type (Δ1 ++ x ~ tt ++ Δ2) τ ->
+    ~ x ∈@ (freeset typ KType τ) ->
+    scoped_type (Δ1 ++ Δ2) τ.
+Proof.
+  introv hyp hnotin. unfold scoped_type in *.
+  eapply stren_scoped; eauto.
+Qed.
+
+Corollary stren_scoped_type_1 : forall Δ x τ,
+    scoped_type (Δ ++ x ~ tt) τ ->
+    ~ x ∈@ (freeset typ KType τ) ->
+    scoped_type Δ τ.
+Proof.
+  introv H1 H2. change_alist (Δ ++ x ~ tt ++ []) in H1.
+  change_alist (Δ ++ []). eauto using stren_scoped_type.
+Qed.
+
+(** The <<scoped_type>> predicate supports substitution w.r.t. in Δ. *)
+Lemma sub_scoped_type : forall Δ1 Δ2 x τ1 τ2,
+    scoped_type (Δ1 ++ x ~ tt ++ Δ2) τ1 ->
+    scoped_type (Δ1 ++ Δ2) τ2 ->
+    scoped_type (Δ1 ++ Δ2) (subst typ KType x τ2 τ1).
+Proof.
+  intros. apply sub_scoped; auto.
+Qed.
+
+Corollary sub_scoped_type_1 : forall Δ x τ1 τ2,
+    scoped_type (Δ ++ x ~ tt) τ1 ->
+    scoped_type Δ τ2 ->
+    scoped_type Δ (subst typ KType x τ2 τ1).
+Proof.
+  introv H1 H2. change_alist (Δ ++ x ~ tt ++ []) in H1.
+  change_alist (Δ ++ []) in H2. change_alist (Δ ++ []).
+  auto using sub_scoped_type.
+Qed.
+
+#[export] Hint Resolve weak_scoped_type_l weak_scoped_type_r perm_scoped_type
+ stren_scoped_type stren_scoped_type_1 sub_scoped_type sub_scoped_type_1 : tea_sysf.
+ *)
+
+(** ** Well-formed type expressions (<<ok_type>>) *)
+(******************************************************************************)
+Corollary ok_type_lc : forall Δ τ,
+    ok_type Δ τ ->
+    locally_closed typ KType τ.
+Proof.
+  unfold ok_type. tauto.
+Qed.
+
+#[export] Hint Resolve ok_type_lc : sysf_ctx.
+
+Lemma perm_ok_type : forall Δ1 Δ2 τ,
+    Permutation Δ1 Δ2 ->
+    ok_type Δ1 τ <->
+    ok_type Δ2 τ.
+Proof.
+  intros. unfold ok_type. rewrite (perm_scoped_iff _ _); eauto.
+  reflexivity.
+Qed.
+
+Lemma perm_ok_type_1 : forall Δ1 Δ2 τ,
+    ok_type Δ1 τ ->
+    Permutation Δ1 Δ2 ->
+    ok_type Δ2 τ.
+Proof.
+  intros. rewrite <- perm_ok_type; eauto.
+Qed.
+
+#[export] Hint Immediate perm_ok_type_1 : sysf_ctx.
+
+(** The <<ok_type>> predicate supports weakening in Δ. *)
+(* TODO: Understand how to prevent
+    auto using weak_scoped_app_l diverges. *)
+Lemma weak_ok_type_r : forall Δ1 Δ2 τ,
+    ok_type Δ1 τ ->
+    ok_type (Δ1 ++ Δ2) τ.
+Proof.
+  unfold ok_type.
+  intros. split.
+  - Check weak_scoped_app_l typ.
+    apply (weak_scoped_app_l typ).
+  - tauto.
+  intuition (eauto using (weak_scoped_app_l typ)).
+Qed.
+
+Lemma weak_ok_type_l : forall Δ1 Δ2 τ,
+    ok_type Δ2 τ ->
+    ok_type (Δ1 ++ Δ2) τ.
+Proof.
+  unfold ok_type. intuition (auto using (weak_scoped_app_r (F:=typ))).
+Qed.
+
+#[export] Hint Resolve weak_ok_type_l weak_ok_type_r : sysf_ctx.
+
+(** The <<ok_type>> predicate supports strengthening in Δ for fresh variables. *)
+Lemma stren_ok_type : forall Δ1 Δ2 x τ,
+    ok_type (Δ1 ++ x ~ tt ++ Δ2) τ ->
+    ~ x ∈@ (freeset typ KType τ) ->
+    ok_type (Δ1 ++ Δ2) τ.
+Proof.
+  introv [? ?] ?. unfold ok_type.
+  eauto using (stren_scoped (F:=typ)).
+Qed.
+
+Corollary stren_ok_type_1 : forall Δ x τ,
+    ok_type (Δ ++ x ~ tt) τ ->
+    ~ x ∈@ (freeset typ KType τ) ->
+    ok_type Δ τ.
+Proof.
+  introv H1 H2. change_alist (Δ ++ x ~ tt ++ []) in H1.
+  change_alist (Δ ++ []). eauto using stren_ok_type.
+Qed.
+
+#[export] Hint Immediate stren_ok_type stren_ok_type_1 : sysf_ctx.
+
+(** The <<ok_type>> predicate supports substitution w.r.t. in Δ. *)
+Lemma sub_ok_type : forall Δ1 Δ2 x τ1 τ2,
+    ok_type (Δ1 ++ x ~ tt ++ Δ2) τ1 ->
+    ok_type (Δ1 ++ Δ2) τ2 ->
+    ok_type (Δ1 ++ Δ2) (subst typ KType x τ2 τ1).
+Proof.
+  unfold ok_type. introv [? ?] [? ?]. split.
+  - auto using (sub_scoped (F:=typ)).
+  - auto using (subst_lc_eq (F:=typ)).
+Qed.
+
+#[export] Hint Resolve sub_ok_type : sysf_ctx.
+
+Corollary sub_ok_type_1 : forall Δ x τ1 τ2,
+    ok_type (Δ ++ x ~ tt) τ1 ->
+    ok_type Δ τ2 ->
+    ok_type Δ (subst typ KType x τ2 τ1).
+Proof.
+  introv H1 H2. change_alist (Δ ++ x ~ tt ++ []) in H1.
+  change_alist (Δ ++ []) in H2. change_alist (Δ ++ []).
+  auto using sub_ok_type.
+Qed.
+
+#[export] Hint Resolve sub_ok_type_1 : sysf_ctx.
+
+(** * Term variable contexts *)
+(** Contexts of <<free term variable, type>> assigments), used to declare free term
+    variables and their associated typee. *)
+(******************************************************************************)
+
+(** A term-variable context <<Γ>> is well formed in type-variable
+    context <<Δ>> when it is duplicate-free and each type is well
+    formed in <<Δ>>. The [ok_tmv] judgment is preserved under
+    permutation of <<Γ>>, and preserved under permutation, weakening,
+    strengthening, and substitution in <<Δ>>.*)
+
+(** ** Structural properties of <<Δ>> in <<ok_tmv Δ Γ>>. *)
+Corollary binds_ok_tmv : forall Δ Γ x τ,
+    ok_tmv Δ Γ ->
+    (x, τ) ∈ Γ ->
+    ok_type Δ τ.
+Proof.
+  introv ? Hin. unfold ok_tmv, ok_type in *.
+  apply binds_in_range in Hin. firstorder.
+Qed.
+
+#[export] Hint Immediate binds_ok_tmv : sysf_ctx.
+
+(** The <<ok_tmv>> predicate supports permutation in Δ. *)
+Theorem perm_ok_tmv : forall Δ1 Δ2 Γ,
+    ok_tmv Δ1 Γ ->
+    Permutation Δ1 Δ2 ->
+    ok_tmv Δ2 Γ.
+Proof.
+  introv [? ?] ?. unfold ok_tmv.
+  split; eauto using perm_ok_type_1 with tea_alist.
+Qed.
+
+#[export] Hint Immediate perm_ok_tmv : sysf_ctx.
+
+Corollary perm_ok_tmv_iff : forall Δ1 Δ2 Γ,
+    Permutation Δ1 Δ2 ->
+    ok_tmv Δ1 Γ <-> ok_tmv Δ2 Γ.
+Proof.
+  introv Hperm. unfold ok_tmv, ok_type.
+  assert (lemma : forall τ, scoped_env typ KType τ Δ1 <->
+                            scoped_env typ KType τ Δ2).
+  { intros. now rewrite perm_scoped_iff. }
+  (* todo : figure out why <<perm_scoped_iff>> won't rewrite by itself. *)
+  setoid_rewrite lemma. firstorder.
+Qed.
+
+(** The <<ok_tmv>> predicate supports weakening in <<Δ>>. *)
+
+#[local] Set Firstorder Depth 4.
+
+Lemma weak_ok_tmv : forall Δ1 Δ2 Γ,
+    ok_tmv Δ1 Γ ->
+    ok_tmv (Δ1 ++ Δ2) Γ.
+Proof.
+  introv [huniq hok1]. unfold ok_tmv in *.
+  firstorder using weak_ok_type_r.
+Qed.
+
+#[export] Hint Resolve weak_ok_tmv : sysf_ctx.
+
+(** The <<ok_tmv>> predicate supports strengthening in <<Δ>> for fresh variables. *)
+Lemma stren_ok_tmv : forall Δ1 Δ2 x Γ,
+    ok_tmv (Δ1 ++ x ~ tt ++ Δ2) Γ ->
+    ~ x ∈@ freeset (fun A => alist typ A) KType Γ ->
+    ok_tmv (Δ1 ++ Δ2) Γ.
+Proof.
+  introv [hunit hok] hfresh. rewrite nin_freeset_iff in hfresh.
+  unfold ok_tmv. split; [trivial |].
+  intros τ hin; specialize (hok τ hin).
+  intuition (eauto using stren_ok_type).
+Qed.
+
+Corollary stren_ok_tmv_1 : forall Δ x Γ,
+    ok_tmv (Δ ++ x ~ tt) Γ ->
+    ~ x ∈@ freeset (fun A => alist typ A) KType Γ ->
+    ok_tmv Δ Γ.
+Proof.
+  introv hyp1 hyp2. change_alist (Δ ++ x ~ tt ++ []) in hyp1.
+  change_alist (Δ ++ []). eauto using stren_ok_tmv.
+Qed.
+
+(** The <<ok_tmv>> predicate supports substitution w.r.t. <<Δ>> *)
+Lemma sub_ok_tmv : forall Δ1 Δ2 x Γ τ,
+    ok_tmv (Δ1 ++ x ~ tt ++ Δ2) Γ ->
+    ok_type (Δ1 ++ Δ2) τ ->
+    locally_closed typ KType τ ->
+    ok_tmv (Δ1 ++ Δ2) (subst (fun A => alist typ A) KType x τ Γ).
+Proof.
+  introv [hunit hok] Hscope lc. unfold ok_tmv. split.
+  - now rewrite <- uniq_subst.
+  - intros τ2 τ2in. rewrite in_range_subst in τ2in.
+    destruct τ2in as [τ2_inv [hin ?]]; subst.
+    specialize (hok τ2_inv hin).
+    auto using sub_ok_type.
+Qed.
+
+#[export] Hint Resolve sub_ok_tmv : sysf_ctx.
+
+(** ** Structural properties of <<Γ>> in <<ok_tmv Δ Γ>>. *)
+
+(** <<ok_tmv Δ Γ>> supports permutation in Γ. *)
+Lemma perm_tm_ok_tmv : forall Δ Γ1 Γ2,
+    ok_tmv Δ Γ1 ->
+    Permutation Γ1 Γ2 ->
+    ok_tmv Δ Γ2.
+Proof.
+  introv [huniq hok]. unfold ok_tmv in *. split.
+  - rewrite uniq_perm; eauto. now symmetry.
+  - intros τ hin; specialize (hok τ).
+    apply hok. rewrite perm_range; eauto.
+Qed.
+
+#[export] Hint Immediate perm_tm_ok_tmv : sysf_ctx.
+
+Corollary perm_tm_ok_tmv_iff : forall Δ Γ1 Γ2,
+    Permutation Γ1 Γ2 ->
+    ok_tmv Δ Γ1 <-> ok_tmv Δ Γ2.
+Proof.
+  introv Hperm; split; intro.
+  - eauto using perm_tm_ok_tmv.
+  - symmetry in Hperm. eauto using perm_tm_ok_tmv.
+Qed.
+
+Lemma ok_tmv_tm_nil : forall Δ,
+    ok_tmv Δ [].
+Proof.
+  intros. unfold ok_tmv in *. now bursts.
+Qed.
+
+#[export] Hint Resolve ok_tmv_tm_nil : sysf_ctx.
+
+Lemma ok_tmv_tm_cons : forall Δ Γ x τ,
+    ok_tmv Δ Γ ->
+    ~ (x ∈@ domset Γ) ->
+    ok_type Δ τ ->
+    ok_tmv Δ (x ~ τ ++ Γ).
+Proof.
+  intros. unfold ok_tmv in *. bursts.
+  splits.
+  - intuition.
+  - intros ? [?|?].
+    + subst. auto.
+    + firstorder.
+Qed.
+
+#[export] Hint Resolve ok_tmv_tm_cons : sysf_ctx.
+
+Lemma ok_tmv_tm_one : forall Δ x τ,
+    ok_type Δ τ ->
+    ok_tmv Δ (x ~ τ).
+Proof.
+  intros. change (x ~ τ) with [(x, τ)].
+  apply ok_tmv_tm_cons; auto using ok_tmv_tm_nil.
+  fsetdec.
+Qed.
+
+#[export] Hint Resolve ok_tmv_tm_one : sysf_ctx.
+
+Lemma ok_tmv_tm_app : forall Δ Γ1 Γ2,
+    ok_tmv Δ (Γ1 ++ Γ2) <->
+    ok_tmv Δ Γ1 /\ ok_tmv Δ Γ2 /\ disjoint Γ1 Γ2.
+Proof.
+  intros. unfold ok_tmv.
+  setoid_rewrite in_range_iff.
+  setoid_rewrite List.in_list_app.
+  rewrite uniq_app_iff. firstorder.
+Qed.
+
+Lemma ok_tmv_inv_app_l : forall Δ Γ1 Γ2,
+    ok_tmv Δ (Γ1 ++ Γ2) ->
+    ok_tmv Δ Γ1.
+Proof.
+  introv [huniq hscope]. unfold ok_tmv in *.
+  bursts. firstorder.
+Qed.
+
+#[export] Hint Immediate ok_tmv_inv_app_l : sysf_ctx.
+
+Lemma ok_tmv_app_comm : forall {Δ Γ1 Γ2},
+    ok_tmv Δ (Γ1 ++ Γ2) <->
+    ok_tmv Δ (Γ2 ++ Γ1).
+Proof.
+  intros. unfold ok_tmv. bursts.
+  rewrite disjoint_sym. firstorder.
+Qed.
+
+#[export] Hint Immediate ok_tmv_app_comm : sysf_ctx.
+
+Corollary ok_tmv_inv_app_r : forall Δ Γ1 Γ2,
+    ok_tmv Δ (Γ1 ++ Γ2) ->
+    ok_tmv Δ Γ2.
+Proof.
+  introv hyp. rewrite ok_tmv_app_comm in hyp.
+  eauto using ok_tmv_inv_app_l.
+Qed.
+
+#[export] Hint Immediate ok_tmv_inv_app_r : sysf_ctx.
+
+Corollary ok_tmv_inv_mid : forall Δ Γ1 Γ2 Γ3,
+    ok_tmv Δ (Γ1 ++ Γ2 ++ Γ3) ->
+    ok_tmv Δ (Γ1 ++ Γ3).
+Proof.
+  introv hyp.
+  change_alist ((Γ1 ++ Γ2) ++ Γ3) in hyp.
+  rewrite ok_tmv_app_comm in hyp.
+  change_alist ((Γ3 ++ Γ1) ++ Γ2) in hyp.
+  apply ok_tmv_inv_app_l in hyp.
+  now rewrite ok_tmv_app_comm in hyp.
+Qed.
+
+#[export] Hint Immediate ok_tmv_inv_mid : sysf_ctx.
+
+(** * Well-formed terms, <<Δ ; Γ ⊢ t OK>> *)
+
+(** ** Structural properties of <<Δ>> in <<Δ ; Γ ⊢ t OK>>. *)
+
+(** ** Structural properties of <<Γ>> in <<Δ ; Γ ⊢ t : τ>>. *)
